Imported the files about separate compilation for the symbol table gen phase

x86/RelocLinking.v
@@ -65,7 +65,7 @@ Definition link_symbtype (t1 t2: symbtype) :=
 (*   | secindex_normal _ , secindex_normal _ => ONone *)
 (*   end. *)
 
-Definition postpone_link_symb (e2: symbentry) : bool :=
+Definition is_symbentry_internal (e2: symbentry) : bool :=
   let i2 := symbentry_secindex e2 in
   match i2 with
   | secindex_undef
@@ -73,15 +73,25 @@ Definition postpone_link_symb (e2: symbentry) : bool :=
   | _ => true
   end.
 
+Definition update_symbtype (e: symbentry) t :=
+  {| symbentry_id    := symbentry_id e;
+     symbentry_bind  := symbentry_bind e;
+     symbentry_type  := t;
+     symbentry_value := symbentry_value e;
+     symbentry_secindex := symbentry_secindex e;
+     symbentry_size  := symbentry_size e; |}.
+
 Definition link_symb (e1 e2: symbentry) : option symbentry :=
   match link_symbtype (symbentry_type e1) (symbentry_type e2) with
   | None => None
-  | Some _ =>
+  | Some t =>
     let sz1 := symbentry_size e1 in
     let sz2 := symbentry_size e2 in
     let i1 := symbentry_secindex e1 in
     let i2 := symbentry_secindex e2 in
     match i1, i2 with
+    | secindex_undef, secindex_undef =>
+      Some (update_symbtype e1 t)
     | _, secindex_undef => Some e1
     | secindex_undef, _ => Some e2
     | _, secindex_comm =>
@@ -116,76 +126,46 @@ Definition reloc_symb (e:symbentry) : option symbentry :=
   | _ => Some e
   end.
 
-Definition reloc_symbtable (t:symbtable) : option symbtable :=
-  fold_right (fun e t =>
-                match t with
-                | None => None
-                | Some t' => 
-                  match reloc_symb e with
-                  | None => None
-                  | Some e' => Some (e' :: t')
-                  end
-                end) 
-             (Some []) t.
-
-
-(** Linking of symbol tables t1 and t2 with the 
-    internal definitions in t2 (denoted by postponed) 
-    appended to after these in t1.
-    We assume t1 and t2 contain symbols with distinct ids *)
-Fixpoint link_symbtable_aux (t1 t2 postponed: symbtable) : option symbtable :=
-  match t1 with
-  | nil => 
-    (** Perform the relocation to the internal definitions in t2 and
-        concatnate them with the unsolved symbols in t2 *)
-    match reloc_symbtable postponed with
+Definition reloc_iter e t :=
+  match t with
+  | None => None
+  | Some t' => 
+    match reloc_symb e with
     | None => None
-    | Some p' =>  Some ((rev p') ++ t2)
-    end
-  | e1 :: t1' => 
-    match symbentry_id e1 with
-    | None => None
-    | Some id1 => 
-      (** e2s contains symbols with the same id as e1 *)
-      let (e2s, t2') := partition (symbentry_id_eq id1) t2 in
-      match e2s with
-      | nil => 
-        (** If there is no symbol with the same id as e1 in t2,
-            then e1 is a distinct symbol. 
-            Perform the rest of the linking and put e1 to the head 
-            of the result *)
-        match link_symbtable_aux t1' t2 postponed with
-        | None => None
-        | Some t => Some (e1 :: t)
-        end
-      | e2::_ =>
-        (** If there is a symbol e2 with the same id as e1 in t2,
-            then link e1 with e2 *)
-        match link_symb e1 e2 with
-        | None => None
-        | Some e3 => 
-          (** If linking of e1 and e2 succeeds, depending on 
-              whether e2 is an internal definition or not,
-              either the result is added to 'postponed' and appended later,
-              or the result made to be the head of the final result *)
-          if postpone_link_symb e2 then
-            link_symbtable_aux t1' t2' (e3 :: postponed)
-          else
-            match (link_symbtable_aux t1' t2' postponed) with
-            | None => None
-            | Some t => Some (e3 :: t)
-            end
-        end
-      end
+    | Some e' => Some (e' :: t')
     end
   end.
-    
-Definition link_symbtable (t1 t2: symbtable) : option symbtable :=
-  let t1' := SeqTable.filter is_not_dummy_symbentry t1 in
-  let t2' := SeqTable.filter is_not_dummy_symbentry t2 in 
-  link_symbtable_aux t1' t2' [].
+
+Definition reloc_symbtable (t:symbtable) : option symbtable :=
+  fold_right reloc_iter (Some []) t.
 
 End WITH_RELOC_OFFSET.
+
+(** Linking of symbol tables *)
+Definition link_symbtable_check (t2: PTree.t symbentry) (x: ident) (symb1: symbentry) :=
+  match t2!x with
+  | None => true
+  | Some symb2 =>
+    match link_symb symb1 symb2 with Some _ => true | None => false end
+  end.
+
+Definition link_symb_merge (o1 o2: option symbentry) :=
+  match o1, o2 with
+  | None, _ => o2
+  | _, None => o1
+  | Some gd1, Some gd2 => link_symb gd1 gd2
+  end.
+
+Definition link_symbtable (t1 t2: symbtable) : option symbtable :=
+  let tree1 := symbtable_to_tree t1 in
+  let tree2 := symbtable_to_tree t2 in
+  if list_norepet_dec ident_eq (get_symbentry_ids t1)
+  && list_norepet_dec ident_eq (get_symbentry_ids t2)
+  && PTree_Properties.for_all tree1 (link_symbtable_check tree2) then
+    let t := PTree.elements (PTree.combine link_symb_merge tree1 tree2) in
+    Some (dummy_symbentry :: map snd t)
+  else
+    None.  
 
 Definition link_section (s1 s2: section) : option section :=
   match s1, s2 with
@@ -219,9 +199,7 @@ Definition link_sectable (s1 s2: sectable) : option sectable :=
     None
   end.
 
-Definition reloc_offset_fun (data_sec code_sec: section): N -> option Z :=
-  let dsz := sec_size data_sec in
-  let csz := sec_size code_sec in
+Definition reloc_offset_fun (dsz csz: Z): N -> option Z :=
   (fun i => if N.eq_dec i (SecIndex.interp sec_data_id) then
            Some dsz
          else if N.eq_dec i (SecIndex.interp sec_code_id) then
@@ -247,24 +225,40 @@ Definition link_reloc_prog (p1 p2: program) : option program :=
     let code_sec1 := SeqTable.get (SecIndex.interp sec_code_id) stbl1 in
     match data_sec1, code_sec1 with
     | Some data_sec1', Some code_sec1' =>
-      let f_rofs := reloc_offset_fun data_sec1' code_sec1' in
       match link_sectable stbl1 stbl2 with
       | None => None
       | Some sectbl =>
-        match link_symbtable f_rofs (prog_symbtable p1) (prog_symbtable p2) with
+        let t1 := (prog_symbtable p1) in
+        let f_rofs := reloc_offset_fun (sec_size data_sec1') (sec_size code_sec1') in
+        match reloc_symbtable f_rofs (prog_symbtable p2) with
         | None => None
-        | Some symbtbl =>
-          Some {| prog_defs   := AST.prog_defs ap;
-                  prog_public := AST.prog_public ap;
-                  prog_main   := AST.prog_main ap;
-                  prog_sectable  := sectbl;
-                  prog_symbtable := symbtbl;
-                  prog_strtable  := prog_strtable p1;
-                  prog_reloctables := prog_reloctables p1;
-                  prog_senv := prog_senv p1; |}
+        | Some t2 =>
+          match link_symbtable t1 t2 with
+          | None => None
+          | Some symbtbl =>
+            Some {| prog_defs   := AST.prog_defs ap;
+                    prog_public := AST.prog_public ap;
+                    prog_main   := AST.prog_main ap;
+                    prog_sectable  := sectbl;
+                    prog_symbtable := symbtbl;
+                    prog_strtable  := prog_strtable p1;
+                    prog_reloctables := prog_reloctables p1;
+                    prog_senv := Globalenvs.Genv.to_senv (Globalenvs.Genv.globalenv ap); |}
+          end
         end
       end
     | _, _ => None
     end
   end.
   
+
+Instance Linker_reloc_prog : Linker program :=
+{
+  link := link_reloc_prog;
+  linkorder := fun _ _ => True;
+}.
+Proof.
+  auto.
+  auto.
+  auto.
+Defined.
