x86/SymbtablegenSep.v
@@ -1,0 +1,2566 @@
+(* ********************* *)
+(* Author: Yuting Wang   *)
+(* Date:   Oct 31, 2019   *)
+(* ********************* *)
+
+Require Import Coqlib Integers AST Maps.
+Require Import Asm.
+Require Import Errors.
+Require Import Memtype.
+Require Import Asm RelocProgram.
+Require Import Symbtablegen.
+Require Import Linking LinkingProp OrderedLinking.
+Require Import RelocLinking.
+Require Import SeqTable.
+Require Import RelationClasses.
+Require Import RelocProgSyneq.
+Import ListNotations.
+
+Set Implicit Arguments.
+
+Local Transparent Linker_def.
+Local Transparent Linker_fundef.
+Local Transparent Linker_vardef.
+Local Transparent Linker_varinit.
+
+Lemma map_pres_subset_rel: forall A B (l1 l2:list A) (f: A -> B),
+    (forall x, In x l1 -> In x l2)
+    -> (forall y, In y (map f l1) -> In y (map f l2)).
+Proof.
+  intros A B l1 l2 f SUB y IN.
+  rewrite in_map_iff in *.
+  destruct IN as (x & EQ & IN). subst.
+  eauto.
+Qed.
+
+Lemma Forall_app_distr: forall A f (l1 l2 : list A),
+    Forall f (l1 ++ l2) 
+    <-> Forall f l1 /\ Forall f l2.
+Proof.
+  induction l1 as [|e l1].
+  - intros l2. cbn. split; auto.
+    tauto.
+  - cbn. intros. generalize (IHl1 l2).
+    destruct 1 as [F1 F2].
+    split.
+    + intros F3. inv F3.
+      generalize (F1 H2). 
+      destruct 1. split; auto.
+    + intros F3. destruct F3 as [F4 F5]. inv F4.
+      auto.
+Qed.
+
+
+Lemma length_S_inv : forall A n (l: list A),
+    length l = S n ->
+    exists l' a, l = l' ++ [a] /\ length l' = n.
+Proof.
+  induction n.
+  - intros. destruct l. cbn in *.
+    congruence.
+    cbn in H. inv H.
+    rewrite length_zero_iff_nil in H1.
+    subst. exists nil. cbn. eauto.
+  - intros. simpl in *. 
+    destruct l. cbn in H. congruence.
+    cbn in H. inv H.
+    generalize (IHn _ H1).
+    destruct 1 as (l' & a0 & eq & LEN). subst.
+    exists (a :: l'). cbn. eexists; split; eauto.
+Qed.
+
+Lemma rev_nil_inv_len : forall A n (l:list A),
+    length l = n -> rev l = [] -> l = nil.
+Proof.
+  induction n.
+  - intros. 
+    rewrite length_zero_iff_nil in H. subst. auto.
+  - intros.
+    generalize (length_S_inv _ H).
+    destruct 1 as (l' & a & EQ & LEN).
+    subst. rewrite rev_unit in H0.
+    inv H0.
+Qed.
+
+Lemma rev_nil_inv : forall A (l:list A),
+    rev l = [] -> l = nil.
+Proof.
+  intros. eapply rev_nil_inv_len; eauto.
+Qed.
+
+Lemma rev_single : forall A (l:list A) a,
+    rev l = [a] -> l = [a].
+Proof.
+  induction l.
+  - cbn in *. congruence.
+  - intros. simpl in H.
+    replace [a0] with (nil ++ [a0]) in H by auto.
+    apply app_inj_tail in H.
+    destruct H; subst. 
+    generalize (rev_nil_inv _ H).
+    intros. subst. auto.
+Qed.
+
+Lemma app_cons_comm : forall (A:Type) (l1 l2: list A) a,
+    l1 ++ (a :: l2) = (l1 ++ [a]) ++ l2.
+Proof.
+  induction l1.
+  - intros. auto.
+  - simpl. intros. rewrite IHl1. auto.
+Qed.
+
+Lemma list_norepet_app: forall A (l1 l2: list A),
+    list_norepet l1 -> list_norepet l2 
+    -> (forall a, In a l1 -> ~ In a l2)
+    -> list_norepet (l1 ++ l2).
+Proof.
+  induction l1; intros until l2; intros NORPT1 NORPT2 EXCL.
+  - cbn. auto.
+  - cbn in *. inv NORPT1.
+    constructor. 
+    + rewrite in_app.
+      intro IN. destruct IN as [IN|IN]; auto.
+      eapply EXCL; eauto.
+    + eapply IHl1; eauto.
+Qed.
+
+Lemma partition_inv_nil1 : forall (A:Type) f (l1 l2:list A),
+    partition f l1 = ([], l2) -> l1 = l2.
+Proof.
+  induction l1; intros; simpl in *.
+  - inv H. auto.
+  - destr_in H. destr_in H. inv H.
+    f_equal. apply IHl1; auto.
+Qed.
+
+Lemma elements_in_partition_prop: forall A f (l l1 l2: list A),
+    partition f l = (l1, l2) -> 
+    (forall x, In x l1 -> f x = true) /\ (forall x, In x l2 -> f x = false).
+Proof.
+  induction l; intros until l2; simpl.
+  - inversion 1. subst. 
+    split; intros; simpl in *; contradiction.
+  - intros PART. destr_in PART. 
+    generalize (IHl _ _ (@eq_refl _ (l0, l3))).
+    destruct 1 as (IN1 & IN2).
+    destr_in PART; inv PART; split; intros; auto.
+    inv H; auto.
+    inv H; auto.
+Qed.
+
+Lemma defs_in_partition_id_not_in : 
+  forall F V (LV: Linker V)
+    id (l l1 l2: list (ident * option (globdef (AST.fundef F) V))),
+    partition (fun '(id', _) => ident_eq id' id) l = (l1, l2) 
+    -> ~ In id (map fst l2).
+Proof. 
+  intros F V LV id l l1 l2 PART.
+  apply elements_in_partition_prop in PART.
+  destruct PART.
+  rewrite in_map_iff. intro IN.
+  destruct IN as (def & EQ & IN3).
+  generalize (H0 _ IN3). destruct def. 
+  inv EQ. cbn. 
+  destruct peq; auto. intros. inv H1.
+Qed.
+
+Lemma part_not_in_nil : forall F V id (defs defs' l: list (ident * option (globdef (AST.fundef F) V))),
+    partition (fun '(id', _) => ident_eq id' id) defs = (l, defs') ->
+    ~ In id (map fst defs) ->
+    l = nil.
+Proof.
+  induction defs. 
+  - intros defs' l PART NIN.
+    simpl in *. inv PART. auto.
+  - intros defs' l PART NIN.
+    simpl in *. destr_in PART. 
+    destruct a, ident_eq; simpl in *; subst; inv PART.
+    exfalso. apply NIN. auto.
+    eapply IHdefs; eauto.
+Qed.
+
+Lemma lst_norepet_partition_inv : forall F V id (defs defs1 defs2: list (ident * option (globdef (AST.fundef F) V))),
+    list_norepet (map fst defs) ->
+    partition (fun '(id', _) => ident_eq id' id) defs = (defs1, defs2) ->
+    defs1 = nil \/ exists def, defs1 = [def].
+Proof.
+  induction defs.
+  - intros defs1 defs2 NORPT PART.
+    simpl in *. inv PART. auto.
+  - intros defs1 defs2 NORPT PART.
+    simpl in *. inv NORPT.
+    destr_in PART. destruct a.
+    destruct ident_eq; simpl in *; inv PART.
+    + generalize (part_not_in_nil _ _ Heqp H1).
+      intros. subst.
+      eauto.
+    + eauto.
+Qed.
+
+Lemma partition_pres_list_norepet : forall F V f (l l1 l2: list (ident * option (globdef (AST.fundef F) V))),
+    partition f l = (l1, l2) -> 
+    list_norepet (map fst l) ->
+    list_norepet (map fst l1) /\ list_norepet (map fst l2).
+Proof.
+  induction l.
+  - intros l1 l2 PART NORPT.
+    simpl in *. inv PART. auto.
+  - intros l1 l2 PART NORPT.
+    simpl in *. inv NORPT. destr_in PART.
+    destr_in PART. 
+    + inv PART.
+      generalize (IHl _ _ (@eq_refl _ (l0, l2)) H2).
+      destruct 1. split; auto. simpl. constructor; auto.
+      intro IN. apply H1. 
+      generalize (elements_in_partition _ _ Heqp).
+      intros ELEM.
+      apply list_in_map_inv in IN. 
+      destruct IN as (b & EQ & IN). 
+      rewrite in_map_iff.
+      exists b.  split; auto.
+      rewrite ELEM. auto.
+    + inv PART.
+      generalize (IHl _ _ (@eq_refl _ (l1, l3)) H2).
+      destruct 1.
+      split; auto.
+      simpl. constructor; auto.
+      intro IN. apply H1.
+      generalize (elements_in_partition _ _ Heqp).
+      intros ELEM.
+      rewrite in_map_iff in *.
+      destruct IN as (x & EQ & IN).
+      eexists; split; eauto.
+      rewrite ELEM. auto.
+Qed.
+
+        
+Lemma get_symbentry_id : forall d_id c_id dsz csz id def,
+    symbentry_id (get_symbentry d_id c_id dsz csz id def) = Some id.
+Proof.
+  intros until def.
+  destruct def. destruct g. destruct f.
+  simpl; auto.
+  simpl; auto.
+  simpl. destruct (gvar_init v); auto. destruct i; auto. destruct l; auto.
+  simpl; auto.
+Qed.
+
+Lemma get_var_entry_size : forall dsz csz id v, 
+    symbentry_size (get_symbentry sec_data_id sec_code_id dsz csz id (Some (Gvar v))) = AST.init_data_list_size (gvar_init v).
+Proof.
+  intros.
+  cbn. destruct (gvar_init v); auto.
+  destruct i; auto.
+  destruct l; auto.
+  cbn. omega.
+Qed.
+
+Lemma get_internal_var_entry : forall dsec csec dsz csz id v,
+    is_var_internal v = true ->
+    get_symbentry dsec csec dsz csz id (Some (Gvar v)) =       
+    {|symbentry_id := Some id;
+      symbentry_bind := get_bind_ty id;
+      symbentry_type := symb_data;
+      symbentry_value := dsz;
+      symbentry_secindex := secindex_normal (SecIndex.interp dsec);
+      symbentry_size := AST.init_data_list_size (AST.gvar_init v);
+    |}.
+Proof.
+  intros dsec csec dsz csz id v INT.
+  unfold is_var_internal in INT.
+  cbn.
+  destruct (gvar_init v); cbn in INT; try congruence.
+  destruct i; cbn in INT; try congruence.
+  destruct l; cbn in INT; try congruence.
+Qed.
+
+Lemma get_comm_var_entry : forall dsec csec dsz csz id v,
+    is_var_comm v = true ->
+    get_symbentry dsec csec dsz csz id (Some (Gvar v)) =       
+    {|symbentry_id := Some id;
+      symbentry_bind := get_bind_ty id;
+      symbentry_type := symb_data;
+      symbentry_value := 8 ; 
+      symbentry_secindex := secindex_comm;
+      symbentry_size := Z.max (AST.init_data_list_size (gvar_init v)) 0;
+    |}.
+Proof.
+  intros dsec csec dsz csz id v INT.
+  unfold is_var_comm in INT.
+  cbn.
+  destruct (gvar_init v); cbn in INT; try congruence.
+  destruct i; cbn in INT; try congruence.
+  destruct l; cbn in INT; try congruence.
+  cbn. f_equal.
+  rewrite Z.add_comm. cbn.
+  rewrite (@Z_max_0 (Z.max z 0)). auto.
+  apply Z.le_ge.
+  apply Z.le_max_r.
+Qed.
+
+Lemma get_external_var_entry : forall dsec csec dsz csz id v,
+    is_var_extern v = true ->
+    get_symbentry dsec csec dsz csz id (Some (Gvar v)) =       
+    {|symbentry_id := Some id;
+      symbentry_bind := get_bind_ty id;
+      symbentry_type := symb_data;
+      symbentry_value := 0;
+      symbentry_secindex := secindex_undef;
+      symbentry_size := 0;
+    |}.
+Proof.
+  intros dsec csec dsz csz id v INT.
+  unfold is_var_extern in INT.
+  cbn.
+  destruct (gvar_init v); cbn in INT; try congruence.
+  destruct i; cbn in INT; try congruence.
+  destruct l; cbn in INT; try congruence.
+Qed.
+
+
+(** * Commutativity of linking and Symbtablgen *)
+
+Definition match_prog (p: Asm.program) (tp: program) :=
+  exists tp', transf_program p = OK tp /\ reloc_prog_syneq tp tp'.
+
+
+Lemma match_prog_pres_prog_defs : forall p tp,
+  match_prog p tp -> AST.prog_defs p = prog_defs tp.
+Proof.
+  intros p tp MATCH. red in MATCH.
+  destruct MATCH as (tp' & MATCH & SEQ).
+  unfold transf_program in MATCH.
+  destruct check_wellformedness; try monadInv MATCH.
+  destruct (gen_symb_table sec_data_id sec_code_id (AST.prog_defs p)) eqn:EQ.
+  destruct p0. 
+  destruct zle; try monadInv MATCH. simpl. auto.
+Qed.
+
+Lemma match_prog_pres_prog_main : forall p tp,
+  match_prog p tp -> AST.prog_main p = prog_main tp.
+Proof.
+  intros p tp MATCH. red in MATCH.
+  destruct MATCH as (tp' & MATCH & SEQ).
+  unfold transf_program in MATCH.
+  destruct check_wellformedness; try monadInv MATCH.
+  destruct (gen_symb_table sec_data_id sec_code_id (AST.prog_defs p)) eqn:EQ.
+  destruct p0. 
+  destruct zle; try monadInv MATCH. simpl. auto.
+Qed.
+
+Lemma match_prog_pres_prog_public : forall p tp,
+  match_prog p tp -> AST.prog_public p = prog_public tp.
+Proof.
+  intros p tp MATCH. red in MATCH.
+  destruct MATCH as (tp' & MATCH & SEQ).
+  unfold transf_program in MATCH.
+  destruct check_wellformedness; try monadInv MATCH.
+  destruct (gen_symb_table sec_data_id sec_code_id (AST.prog_defs p)) eqn:EQ.
+  destruct p0. 
+  destruct zle; try monadInv MATCH. simpl. auto.
+Qed.
+
+  
+Lemma eq_gvar_init_pres_aligned : forall v1 v2,
+    gvar_init v1 = gvar_init v2 
+    -> def_aligned (Some (Gvar v1))
+    -> def_aligned (Some (Gvar v2)).
+Proof.
+  intros. cbn in *. rewrite <- H.
+  auto.
+Qed.
+
+Lemma link_varinit_internal_external_pres_aligned:
+  forall (v1 v2: globvar unit) l inf rd vl,
+    is_var_internal v2 = false
+    -> def_aligned (Some (Gvar v1))
+    -> link_varinit (gvar_init v1) (gvar_init v2) = Some l
+    -> def_aligned (Some (Gvar (mkglobvar inf l rd vl))).
+Proof.
+  intros v1 v2 l inf rd vl INT2 ALIGN LINK.
+  destruct (is_var_internal v1) eqn:INT1.
+  - generalize (link_internal_external_varinit _ _ _ INT1 INT2 LINK).
+    destruct 1 as (EQ & CLS). subst.   
+    apply eq_gvar_init_pres_aligned with v1; auto.
+  - generalize (link_external_varinit _ _ _ INT1 INT2 LINK).
+    intros CLS.
+    destruct l. cbn. auto.
+    cbn in *. destruct i; try congruence.
+    destruct l; try congruence. auto.
+Qed.
+
+
+Lemma link_vardef_internal_external_pres_aligned:
+  forall v1 v2 v,
+    is_var_internal v2 = false
+    -> def_aligned (Some (Gvar v1))
+    -> link_vardef v1 v2 = Some v
+    -> def_aligned (Some (Gvar v)).
+Proof.
+  intros v1 v2 v INT ALIGN LINK.
+  unfold link_vardef in LINK. 
+  destr_in LINK; try congruence.
+  destr_in LINK; try congruence.
+  destr_in LINK; try congruence.
+  inv LINK. unfold is_var_internal in INT.
+  eapply link_varinit_internal_external_pres_aligned; eauto.
+Qed.
+  
+
+Lemma external_var_aligned: forall v,
+    is_var_internal v = false -> def_aligned (Some (Gvar v)).
+Proof.
+  intros v INT.
+  unfold is_var_internal in INT.
+  cbn. destruct (gvar_init v); cbn in *; try congruence.
+  auto.
+  destruct i; cbn in *; try congruence.
+  destruct l; cbn in *; try congruence.
+  auto.
+Qed.
+
+
+Lemma link_option_internal_external_pres_aligned: forall def1 def2 def,
+    is_def_internal is_fundef_internal def2 = false
+    -> def_aligned def1
+    -> link_option def1 def2 = Some def
+    -> def_aligned def.
+Proof.
+  intros def1 def2 def INT ALIGN LINK.
+  destruct def2. destruct g. destruct f; cbn in *; try congruence.
+  - destruct def1. destruct g. destruct f. 
+    + cbn in LINK. destr_in LINK; try congruence. inv LINK.
+      destr_in Heqo; try congruence; inv Heqo.
+      destruct e; try congruence. inv Heqo0. auto.
+    + cbn in LINK. destr_in LINK; try congruence. inv LINK.
+      destr_in Heqo; try congruence; inv Heqo.
+      destr_in Heqo0; try congruence. 
+    + cbn in LINK. congruence.
+    + cbn in LINK. inv LINK. auto.
+  - destruct def1. destruct g.
+    + cbn in *. congruence.
+    + cbn in LINK. destr_in LINK; try congruence.
+      destr_in Heqo; try congruence. inv Heqo. inv LINK.
+      cbn in INT.
+      eapply link_vardef_internal_external_pres_aligned; eauto.
+    + cbn in *. inv LINK.       
+      eapply external_var_aligned; eauto.
+  - destruct def1. cbn in LINK. inv LINK. auto.
+    cbn in *. inv LINK. auto.
+Qed.
+     
+
+(** ** Commutativity of linking and generation of the symbol table *)
+
+
+Lemma acc_symb_append : forall d_id c_id defs dsz1 csz1 stbl1 dsz2 csz2 stbl2 stbl3,
+    fold_left (acc_symb d_id c_id) defs (stbl1, dsz1, csz1) = (stbl2, dsz2, csz2) ->
+    fold_left (acc_symb d_id c_id) defs (stbl1 ++ stbl3, dsz1, csz1) = (stbl2 ++ stbl3, dsz2, csz2).
+Proof.
+  induction defs.
+  - intros until stbl2. intros stbl3 ACC. simpl in *.
+    inv ACC. auto.
+  - intros until stbl2. intros stbl3 ACC. simpl in *.
+    destr_in ACC. destruct a. inv Heqp. destr_in ACC.
+    rewrite app_comm_cons.
+    apply IHdefs. auto.
+Qed.
+
+Lemma acc_symb_append_nil : forall d_id c_id defs dsz1 csz1 dsz2 csz2 stbl2 stbl3,
+    fold_left (acc_symb d_id c_id) defs ([], dsz1, csz1) = (stbl2, dsz2, csz2) ->
+    fold_left (acc_symb d_id c_id) defs (stbl3, dsz1, csz1) = (stbl2 ++ stbl3, dsz2, csz2).
+Proof.
+  intros until stbl3. intros ACC.
+  replace stbl3 with ([] ++ stbl3) by auto.
+  apply acc_symb_append. auto.
+Qed.
+
+
+Lemma acc_symb_inv: forall asf d_id c_id defs stbl1 dsz1 csz1 stbl2 dsz2 csz2,
+    asf = (acc_symb d_id c_id) ->
+    fold_left asf defs (stbl1, dsz1, csz1) = (stbl2, dsz2, csz2) ->
+    exists stbl1', stbl2 = stbl1' ++ stbl1 /\
+              fold_left asf defs ([], dsz1, csz1) = (stbl1', dsz2, csz2).
+Proof.
+  induction defs.
+  - intros stbl1 dsz1 csz1 stbl2 dsz2 csz2 ASF ACC.
+    simpl in *. inv ACC. exists nil. eauto.
+  - intros until csz2. intros ASF ACC. simpl in *.
+    rewrite ASF in ACC. simpl in ACC. destruct a as (id & def).
+    destruct (update_code_data_size dsz1 csz1 def) as [dsize' csize'] eqn:UPDATE.
+    rewrite <- ASF in ACC.
+    generalize (IHdefs _ _ _ _ _ _ ASF ACC).
+    destruct 1 as (stbl1' & EQ & ACC1).
+    rewrite app_cons_comm in EQ.
+    rewrite EQ.
+    eexists. split; auto.
+    subst. simpl.
+    rewrite UPDATE. 
+    apply acc_symb_append_nil. auto.
+Qed.
+
+Definition symbentry_index_in_range range e :=
+  match symbentry_secindex e with
+  | secindex_normal i => In i range
+  | _ => True
+  end.
+
+Definition symbtable_indexes_in_range range t :=
+  Forall (symbentry_index_in_range range) t.
+
+Lemma get_symbentry_in_range: forall d_id c_id dsz csz id def,
+  symbentry_index_in_range [SecIndex.interp d_id; SecIndex.interp c_id] (get_symbentry d_id c_id dsz csz id def).
+Proof.
+  intros.
+  destruct def. destruct g. destruct f.
+  - cbn. auto.
+  - cbn. auto.
+  - destruct (is_var_internal v) eqn:INT.
+    + rewrite get_internal_var_entry; auto. cbn. auto.
+    + rewrite var_not_internal_iff in INT.
+      destruct INT as [INT | INT].
+      * rewrite get_comm_var_entry; auto. cbn. auto.
+      * rewrite get_external_var_entry; auto. cbn. auto.
+  - cbn. auto.
+Qed.
+
+Lemma acc_symb_index_in_range: forall d_id c_id defs dsz1 csz1 tbl dsz2 csz2,
+      fold_left (acc_symb d_id c_id) defs ([], dsz1, csz1) = (tbl, dsz2, csz2)
+      -> symbtable_indexes_in_range (map SecIndex.interp [d_id; c_id]) (rev tbl).
+Proof.
+  induction defs as [| def defs].
+  - intros until csz2. intros ACC. cbn in *.
+    inv ACC. red. cbn. apply Forall_nil.
+  - intros until csz2. intros ACC. cbn in *.
+    destruct def as [id def]. destr_in ACC.
+    generalize (acc_symb_inv _ _ _ _ eq_refl ACC).
+    destruct 1 as (stbl1' & EQ & ACC'). subst.
+    rewrite rev_unit.
+    generalize (IHdefs _ _ _ _ _ ACC').
+    intros IN_RNG.
+    red. rewrite Forall_forall.
+    intros x IN.
+    inv IN.
+    + apply get_symbentry_in_range.
+    + red in IN_RNG.
+      rewrite Forall_forall in IN_RNG.
+      apply IN_RNG; auto.
+Qed.
+
+Lemma gen_symb_table_index_in_range : forall defs sec_data_id sec_code_id stbl dsz csz,
+    gen_symb_table sec_data_id sec_code_id defs = (stbl, dsz, csz) ->
+    symbtable_indexes_in_range (map SecIndex.interp [sec_data_id; sec_code_id]) stbl.
+Proof.
+  intros until csz.
+  intros GS.
+  unfold gen_symb_table in GS. destr_in GS. destruct p. inv GS.
+(*   eapply acc_symb_index_in_range; eauto. *)
+(* Qed. *)
+Admitted.
+
+Lemma reloc_symbentry_exists: forall e dsz csz,
+  symbentry_index_in_range (map SecIndex.interp [sec_data_id; sec_code_id]) e ->
+  exists e', reloc_symb (reloc_offset_fun dsz csz) e = Some e'.
+Proof.
+  intros e dsz csz IN.
+  red in IN. unfold reloc_symb.
+  destruct (symbentry_secindex e); eauto.
+  cbn in IN.
+  unfold reloc_offset_fun.
+  destruct IN as [IN|IN].
+  - rewrite IN. destruct N.eq_dec; try congruence. subst.
+    eauto.
+  - destruct IN as [IN|IN]; try contradiction. subst.
+    destruct N.eq_dec. unfold SecIndex.interp in e0. inv e0.
+    destruct N.eq_dec; try congruence. subst.
+    eauto.
+Qed.
+
+Lemma reloc_symbtable_exists_aux : forall stbl f dsz csz,
+    symbtable_indexes_in_range (map SecIndex.interp [sec_data_id; sec_code_id]) stbl ->
+    f = (reloc_offset_fun dsz csz) ->
+    exists stbl', reloc_symbtable f stbl = Some stbl' /\
+             Forall2 (fun e1 e2 => reloc_symb f e1 = Some e2) stbl stbl'.
+Proof.
+  induction stbl as [|e stbl].
+  - intros f dsz csz INRNG eq. subst.
+    cbn. eexists; eauto.
+  - intros f dsz csz INRNG eq. subst.
+    inv INRNG.
+    generalize (IHstbl _ dsz csz H2 eq_refl).
+    destruct 1 as (stbl' & RELOC & INRNG').
+    unfold reloc_symbtable.
+    cbn. setoid_rewrite RELOC.
+    unfold reloc_iter.
+    generalize (reloc_symbentry_exists _ dsz csz H1).
+    destruct 1 as (e' & RELOC').
+    rewrite RELOC'. eexists; split; eauto.
+Qed.
+
+Lemma reloc_symbtable_exists: forall stbl f defs d c dsz csz,
+    gen_symb_table sec_data_id sec_code_id defs = (stbl, d, c) ->
+    f = (reloc_offset_fun dsz csz) ->
+    exists stbl', reloc_symbtable f stbl = Some stbl' /\
+             Forall2 (fun e1 e2 => reloc_symb f e1 = Some e2) stbl stbl'.
+Proof.
+  intros. apply reloc_symbtable_exists_aux with dsz csz.
+  eapply gen_symb_table_index_in_range; eauto.
+  auto.
+Qed.
+
+Lemma update_code_data_size_external_size_inv : forall def1 dsz1 csz1 dsz1' csz1',
+    is_def_internal is_fundef_internal def1 = false ->
+    update_code_data_size dsz1 csz1 def1 = (dsz1', csz1') ->
+    dsz1' = dsz1 /\ csz1' = csz1.
+Proof.
+  intros def1 dsz1 csz1 dsz1' csz1' INT UPDATE.
+  destruct def1. destruct g. destruct f.
+  - simpl in *. congruence.
+  - simpl in *. inv UPDATE. auto.
+  - simpl in INT.
+    unfold is_var_internal in INT.
+    unfold update_code_data_size in UPDATE.
+    destruct (gvar_init v).
+    + simpl in *. inv UPDATE. auto.
+    + destruct i; try (simpl in INT; congruence).
+      simpl in INT. destruct l.
+      * inv UPDATE. auto.
+      * congruence.
+  - simpl in *. inv UPDATE. auto.
+Qed.
+
+Lemma update_code_data_size_external_ignore_size : forall def1 dsz1 csz1,
+    is_def_internal is_fundef_internal def1 = false ->
+    update_code_data_size dsz1 csz1 def1 = (dsz1, csz1).
+Proof.
+  intros def1 dsz1 csz1 INT.
+  destruct def1. destruct g.
+  destruct f; cbn in INT; try congruence.
+  - cbn. auto.
+  - cbn in INT.
+    unfold update_code_data_size.
+    unfold is_var_internal in INT.
+    destruct (gvar_init v); cbn in INT; try congruence.
+    destruct i; cbn in INT; try congruence.
+    destruct l; cbn in INT; try congruence.
+  - cbn. auto.
+Qed.
+
+Lemma get_extern_symbentry_ignore_size: forall id def dsz1 csz1 dsz2 csz2,
+    is_def_internal is_fundef_internal def = false ->
+    get_symbentry sec_data_id sec_code_id dsz1 csz1 id def =
+    get_symbentry sec_data_id sec_code_id dsz2 csz2 id def.
+Proof.
+  intros until csz2. intros INT.
+  destruct def. destruct g. destruct f.
+  - cbn in *. congruence.
+  - cbn in *. auto.
+  - cbn in *. unfold is_var_internal in INT.
+    destruct (gvar_init v); cbn in *; auto.
+    destruct i; try congruence.
+    destruct l; auto.
+    congruence.
+  - cbn in *. auto.
+Qed.
+
+Lemma acc_symb_partition_extern_intern: forall asf id defs defs1 defs2 rstbl dsz1 csz1 dsz2 csz2,
+    asf = acc_symb sec_data_id sec_code_id ->
+    partition (fun '(id', _) => ident_eq id' id) defs = (defs1, defs2) ->
+    fold_left asf defs ([], dsz1, csz1) = (rstbl, dsz2, csz2) ->
+    Forall (fun '(id', def) => is_def_internal is_fundef_internal def = false) defs1 ->
+    exists stbl1 stbl2,
+      partition (symbentry_id_eq id) (rev rstbl) = (stbl1, stbl2) /\
+      fold_left asf defs1 ([], 0, 0) = (rev stbl1, 0, 0) /\
+      fold_left asf defs2 ([], dsz1, csz1) = (rev stbl2, dsz2, csz2).
+Proof.
+  induction defs as [|def defs].
+  - intros until csz2.
+    intros ASF PART ACC EXT.
+    simpl in *. inv PART. inv ACC. simpl.
+    eauto.
+  - intros until csz2.
+    intros ASF PART ACC EXT.
+    simpl in *. destr_in PART. destruct def as (id' & def).
+    destruct ident_eq; subst.
+    + simpl in *. destr_in ACC. inv PART.
+      generalize (acc_symb_inv _ _ _ _ eq_refl ACC).
+      destruct 1 as (rstbl' & EQ & ACC'). subst.
+      inv EXT.
+      generalize (IHdefs _ _ _ _ _ _ _ eq_refl eq_refl ACC' H2).
+      destruct 1 as (stbl1' & stbl2' & PART' & ACC'' & ACC''').
+      rewrite rev_unit. simpl.
+      rewrite PART'.
+      unfold symbentry_id_eq. rewrite get_symbentry_id.
+      rewrite dec_eq_true.
+      do 2 eexists; split; auto. 
+      generalize (update_code_data_size_external_size_inv _ _ _ H1 Heqp0).
+      destruct 1; subst. 
+      split; auto.
+      generalize (update_code_data_size_external_ignore_size def 0 0 H1).
+      intros UPDATE'. rewrite UPDATE'.
+      simpl. 
+      rewrite (get_extern_symbentry_ignore_size id def dsz1 csz1 0 0); auto.
+      apply acc_symb_append_nil. auto.
+    + simpl in *. destr_in ACC. inv PART.
+      generalize (acc_symb_inv _ _ _ _ eq_refl ACC).
+      destruct 1 as (rstbl' & EQ & ACC'). subst.
+      generalize (IHdefs _ _ _ _ _ _ _ eq_refl eq_refl ACC' EXT).
+      destruct 1 as (stbl1' & stbl2' & PART' & ACC'' & ACC''').
+      rewrite rev_unit. simpl.
+      rewrite PART'.
+      unfold symbentry_id_eq. rewrite get_symbentry_id.
+      rewrite dec_eq_false; auto.
+      do 2 eexists; split; auto.
+      rewrite Heqp0. 
+      split; auto.
+      apply acc_symb_append_nil. auto.
+Qed.
+      
+      
+Definition match_def_symbentry (id_def: ident * option gdef) e :=
+  let '(id, def) := id_def in
+  exists dsz csz, e = get_symbentry sec_data_id sec_code_id dsz csz id def.
+    
+Lemma acc_symb_pres_partition: forall asf id defs defs1 defs2 rstbl dsz1 csz1 dsz2 csz2,
+    asf = acc_symb sec_data_id sec_code_id ->
+    partition (fun '(id', _) => ident_eq id' id) defs = (defs1, defs2) ->
+    fold_left asf defs ([], dsz1, csz1) = (rstbl, dsz2, csz2) ->
+    exists stbl1 stbl2,
+      partition (symbentry_id_eq id) (rev rstbl) = (stbl1, stbl2) /\
+      Forall2 match_def_symbentry defs1 stbl1  /\
+      Forall2 match_def_symbentry defs2 stbl2.
+Proof.
+  induction defs as [|def defs].
+  - intros until csz2. 
+    intros ASF PART ACC.
+    simpl in *. inv PART. inv ACC. simpl. eauto.
+  - intros until csz2.
+    intros ASF PART ACC. subst.
+    simpl in *.
+    destruct def as (id', def).
+    destr_in PART. destr_in ACC.
+    generalize (acc_symb_inv _ _ _ _ eq_refl ACC).
+    destruct 1 as (rstbl' & EQ & ACC'). subst.
+    destruct ident_eq; inv PART; simpl in *.
+    + rewrite rev_unit.
+      generalize (IHdefs _ _ _ _ _ _ _ eq_refl eq_refl ACC').
+      destruct 1 as (stbl1' & stbl2' & PART' & MATCH1 & MATCH2).
+      simpl. rewrite PART'.
+      unfold symbentry_id_eq. 
+      rewrite get_symbentry_id. 
+      rewrite dec_eq_true.
+      do 2 eexists; split; eauto.
+      split; auto.
+      constructor; auto.
+      red. eauto.
+    + rewrite rev_unit.
+      generalize (IHdefs _ _ _ _ _ _ _ eq_refl eq_refl ACC').
+      destruct 1 as (stbl1' & stbl2' & PART' & MATCH1 & MATCH2).
+      simpl. rewrite PART'.
+      unfold symbentry_id_eq. 
+      rewrite get_symbentry_id. 
+      rewrite dec_eq_false; auto.
+      do 2 eexists; split; eauto.
+      split; auto.
+      constructor; auto.
+      red. eauto.
+Qed.      
+
+
+Lemma get_symbentry_pres_internal_prop : forall id dsz csz def,
+    is_def_internal is_fundef_internal def = 
+    is_symbentry_internal (get_symbentry sec_data_id sec_code_id dsz csz id def).
+Proof.
+  intros. destruct def.
+  destruct g. destruct f.
+  - cbn. auto.
+  - cbn. auto.
+  - cbn. unfold is_var_internal. 
+    destruct (gvar_init v); cbn; auto.
+    destruct i; cbn; auto.
+    destruct l; cbn; auto.
+  - cbn. auto.
+Qed.
+
+Lemma match_def_symbentry_pres_internal_prop : forall id def e,
+    match_def_symbentry (id, def) e ->
+    is_def_internal is_fundef_internal def = is_symbentry_internal e.
+Proof.
+  intros id def e MATCH.
+  red in MATCH. destruct MATCH as (dsz & csz & SYMB). subst.
+  apply get_symbentry_pres_internal_prop.
+Qed.
+
+
+
+Lemma get_var_entry_type : forall dsz1 csz1 id v,
+    symbentry_type (get_symbentry sec_data_id sec_code_id dsz1 csz1 id (Some (Gvar v))) = symb_data.
+Proof.
+  intros. cbn.
+  destruct (gvar_init v); auto.
+  destruct i; auto.
+  destruct l; auto.
+Qed.
+
+Lemma get_fun_entry_type : forall dsz1 csz1 id f,
+    symbentry_type (get_symbentry sec_data_id sec_code_id dsz1 csz1 id (Some (Gfun f))) = symb_func.
+Proof.
+  intros. cbn.
+  destruct f; auto.
+Qed.
+
+Lemma get_none_entry_type : forall dsz1 csz1 id,
+    symbentry_type (get_symbentry sec_data_id sec_code_id dsz1 csz1 id None) = symb_notype.
+Proof.
+  intros. cbn. auto.
+Qed.
+
+Lemma get_none_entry_secindex : forall dsz1 csz1 id,
+    symbentry_secindex (get_symbentry sec_data_id sec_code_id dsz1 csz1 id None) = secindex_undef.
+Proof.
+  intros. cbn. auto.
+Qed.
+
+Lemma get_extfun_entry_secindex : forall dsz1 csz1 id f,
+    is_fundef_internal f = false 
+    -> symbentry_secindex (get_symbentry sec_data_id sec_code_id dsz1 csz1 id (Some (Gfun f))) = secindex_undef.
+Proof.
+  intros. cbn. auto.
+  destruct f.
+  cbn in *. congruence.
+  simpl. auto.
+Qed.
+
+Lemma get_comm_var_entry_secindex:
+  forall (dsz1 csz1 : Z) (id : ident) v,
+  is_var_comm v = true 
+  -> symbentry_secindex
+      (get_symbentry sec_data_id sec_code_id dsz1 csz1 id
+                         (Some (Gvar v))) = secindex_comm.
+Proof.
+  intros. subst. cbn. 
+  unfold is_var_comm in H.
+  destruct (gvar_init v); cbn in H; try congruence.
+  cbn. auto.
+  destruct i; cbn in H; try congruence.
+  destruct l; cbn in H; try congruence.
+  cbn. auto.
+Qed.
+
+Lemma get_extern_var_entry_secindex:
+  forall (dsz1 csz1 : Z) (id : ident) v,
+  is_var_extern v = true 
+  -> symbentry_secindex
+          (get_symbentry sec_data_id sec_code_id dsz1 csz1 id
+                         (Some (Gvar v))) = secindex_undef.
+Proof.
+  intros. subst. cbn. 
+  unfold is_var_extern in H.
+  destruct (gvar_init v); cbn in H; try congruence.
+  cbn. auto.
+  destruct i; cbn in H; try congruence.
+  destruct l; cbn in H; try congruence.
+Qed.
+
+
+Lemma get_intvar_entry_secindex:
+  forall (dsz1 csz1 : Z) (id : ident) v,
+  is_var_internal v = true 
+  -> symbentry_secindex
+          (get_symbentry sec_data_id sec_code_id dsz1 csz1 id
+                         (Some (Gvar v))) = 
+    (secindex_normal (SecIndex.interp sec_data_id)).
+Proof.
+  intros. cbn.
+  unfold is_var_internal in H.
+  destruct (gvar_init v); cbn in H; try congruence.
+  destruct i; cbn in *; try congruence.
+  destruct l; cbn in *; try congruence.
+Qed.
+
+
+(* Lemma symbentry_secindex_dec : forall e, *)
+(*     {symbentry_secindex e = secindex_undef} + *)
+(*     {symbentry_secindex e <> secindex_undef}. *)
+(* Proof. *)
+(*   decide equality. *)
+(*   apply N.eq_dec. *)
+(* Qed. *)
+
+Lemma update_symbtype_unchanged: forall e t,
+    symbentry_type e = t -> update_symbtype e t = e.
+Proof.
+  intros. destruct e. cbn in *.
+  unfold update_symbtype. cbn. rewrite H. auto.
+Qed.
+
+Lemma link_get_symbentry_left_some_right_none_comm: forall def id dsz1 dsz2 csz1 csz2,
+    link_symb (get_symbentry sec_data_id sec_code_id dsz1 csz1 id (Some def))
+              (get_symbentry sec_data_id sec_code_id dsz2 csz2 id None) = 
+    Some (get_symbentry sec_data_id sec_code_id dsz1 csz1 id (Some def)).
+Proof.
+  intros until csz2.
+  destruct def. destruct f.
+  - cbn. auto.
+  - cbn. auto.
+  - unfold link_symb.
+    rewrite get_var_entry_type.
+    rewrite get_none_entry_type.
+    replace (link_symbtype symb_data symb_notype) with (Some symb_data) by auto.
+    rewrite get_none_entry_secindex.
+    destruct (symbentry_secindex
+                (get_symbentry sec_data_id sec_code_id dsz1 csz1 id
+                               (Some (Gvar v)))); auto.
+    f_equal. apply update_symbtype_unchanged.
+    apply get_var_entry_type.
+Qed.      
+
+
+Lemma link_get_symbentry_right_none_comm: forall def1 def id dsz1 dsz2 csz1 csz2,
+    link_option def1 None = Some def 
+    -> link_symb (get_symbentry sec_data_id sec_code_id dsz1 csz1 id def1)
+                (get_symbentry sec_data_id sec_code_id dsz2 csz2 id None) = 
+      Some (get_symbentry sec_data_id sec_code_id dsz1 csz1 id def).
+Proof.
+  intros until csz2.
+  intros LINK.
+  unfold link_option in LINK.
+  destruct def1 as [def1|].
+  - inv LINK.    
+    eapply link_get_symbentry_left_some_right_none_comm; eauto.
+  - inv LINK. cbn. auto.
+Qed.
+
+Lemma link_get_symbentry_right_extfundef_comm: forall id f1 f2 f dsz1 csz1 dsz2 csz2,
+    is_fundef_internal f2 = false
+    -> link_fundef f1 f2 = Some f
+    -> link_symb
+        (get_symbentry sec_data_id sec_code_id dsz1 csz1 id
+                       (Some (Gfun f1)))
+        (get_symbentry sec_data_id sec_code_id dsz2 csz2 id
+                       (Some (Gfun f2))) =
+      Some (get_symbentry sec_data_id sec_code_id dsz1 csz1 id
+                          (Some (Gfun f))).
+Proof.
+  intros until csz2.
+  intros INT LINK.
+  unfold link_symb.
+  rewrite get_fun_entry_type.
+  rewrite get_fun_entry_type.
+  cbn -[get_symbentry].
+  rewrite (get_extfun_entry_secindex _ _ _ f2); auto.
+
+  destruct f2; try (cbn in INT; congruence).
+  apply link_fundef_inv1 in LINK. subst.
+  destr; auto.
+  f_equal. apply update_symbtype_unchanged.
+  apply get_fun_entry_type.
+Qed.
+
+Lemma link_getsymbentry_right_extfun : forall id def1 def f dsz1 csz1 dsz2 csz2,
+    is_fundef_internal f = false
+    -> link_option def1 (Some (Gfun f)) = Some def
+    -> link_symb
+        (get_symbentry sec_data_id sec_code_id dsz1 csz1 id def1)
+        (get_symbentry sec_data_id sec_code_id dsz2 csz2 id (Some (Gfun f))) =
+      Some (get_symbentry sec_data_id sec_code_id dsz1 csz1 id def).
+Proof.
+  intros until csz2.
+  intros INT LINK.
+  destruct def1 as [def1|].
+  - inv LINK.
+    destr_in H0; try congruence. inv H0.
+    destruct def1; try (cbn in *; congruence).
+    simpl in Heqo. destr_in Heqo; try congruence.
+    inv Heqo.
+    apply link_get_symbentry_right_extfundef_comm; auto.    
+  - inv LINK. 
+    unfold link_symb.   
+    rewrite get_fun_entry_type.
+    rewrite get_none_entry_type.
+    replace (link_symbtype symb_notype symb_func) with (Some symb_func) by auto.
+    rewrite get_none_entry_secindex.
+    rewrite get_extfun_entry_secindex; auto.
+    unfold update_symbtype. cbn. 
+    destruct f. cbn in *; congruence. auto.
+Qed.
+
+
+Lemma link_get_symbentry_extvars_init_comm :
+  forall v1 v2 id dsz1 csz1 dsz2 csz2 (inf:unit) init rd vl,
+    is_var_internal v1 = false 
+    -> is_var_internal v2 = false 
+    -> link_varinit (gvar_init v1) (gvar_init v2) = Some init
+    -> link_symb
+        (get_symbentry sec_data_id sec_code_id dsz1 csz1 id
+                       (Some (Gvar v1)))
+        (get_symbentry sec_data_id sec_code_id dsz2 csz2 id
+                       (Some (Gvar v2))) =
+      Some
+        (get_symbentry sec_data_id sec_code_id dsz1 csz1 id
+                       (Some (Gvar (mkglobvar inf init rd vl)))).
+Proof.
+  intros until vl.
+  intros INT1 INT2 LINK.
+  rewrite var_not_internal_iff in INT1, INT2.
+  destruct INT1 as [INT1|INT1]; destruct INT2 as [INT2|INT2].
+  - generalize (link_comm_vars_init _ _ INT1 INT2 LINK).
+    destruct 1 as (EQ & INIT). subst.
+    repeat (rewrite get_comm_var_entry; auto).
+    cbn.
+    rewrite EQ.
+    destruct zeq; try congruence.
+  - generalize (link_comm_extern_var_init _ _ INT1 INT2 LINK).
+    intros. subst.
+    rewrite (get_comm_var_entry _ _ _ _ _ _ INT1).
+    rewrite (get_external_var_entry _ _ _ _ _ _ INT2).
+    rewrite get_comm_var_entry; auto.
+  - generalize (link_extern_comm_var_init _ _ INT1 INT2 LINK).
+    intros. subst.
+    rewrite (get_comm_var_entry _ _ _ _ _ _ INT2).
+    rewrite (get_external_var_entry _ _ _ _ _ _ INT1).
+    rewrite get_comm_var_entry; auto.
+  - generalize (link_extern_vars_init _ _ INT1 INT2 LINK).
+    intros. subst.
+    rewrite (get_external_var_entry _ _ _ _ _ _ INT2).
+    rewrite (get_external_var_entry _ _ _ _ _ _ INT1).
+    rewrite get_external_var_entry; auto.
+Qed.    
+    
+
+Lemma link_get_symbentry_right_extvar_init_comm :
+  forall v1 v2 id dsz1 csz1 dsz2 csz2 (inf:unit) init rd vl,
+    is_var_internal v2 = false 
+    -> link_varinit (gvar_init v1) (gvar_init v2) = Some init
+    -> link_symb
+        (get_symbentry sec_data_id sec_code_id dsz1 csz1 id
+                       (Some (Gvar v1)))
+        (get_symbentry sec_data_id sec_code_id dsz2 csz2 id
+                       (Some (Gvar v2))) =
+      Some
+        (get_symbentry sec_data_id sec_code_id dsz1 csz1 id
+                       (Some (Gvar (mkglobvar inf init rd vl)))).
+Proof.
+  intros until vl.
+  intros INT LINK.
+  destruct (is_var_internal v1) eqn:INT1.
+  generalize INT. intros INT'.
+  rewrite var_not_internal_iff in INT.
+  destruct INT as [INT|INT].
+  - generalize (link_internal_comm_varinit _ _ _ INT1 INT LINK).
+    destruct 1 as (IEQ & SEQ & CLS1). subst.
+    unfold link_symb.
+    repeat rewrite get_var_entry_type.
+    cbn -[get_symbentry].
+    rewrite get_intvar_entry_secindex; auto.
+    rewrite get_comm_var_entry_secindex; auto.
+    rewrite get_var_entry_size.
+    rewrite get_var_entry_size.
+    rewrite SEQ.
+    apply dec_eq_true. 
+  - unfold link_symb.
+    repeat rewrite get_var_entry_type.
+    cbn -[get_symbentry].
+    rewrite get_intvar_entry_secindex; auto.
+    rewrite get_extern_var_entry_secindex; auto.
+    generalize (link_internal_external_varinit _ _ _ INT1 INT' LINK).
+    destruct 1 as (INITEQ & CLS).
+    f_equal. cbn. rewrite INITEQ. auto.
+  - apply link_get_symbentry_extvars_init_comm; auto.
+Qed.
+    
+
+Lemma link_getsymbentry_right_extvar : forall id def1 def v dsz1 csz1 dsz2 csz2,
+    is_var_internal v = false
+    -> link_option def1 (Some (Gvar v)) = Some def
+    -> link_symb
+        (get_symbentry sec_data_id sec_code_id dsz1 csz1 id def1)
+        (get_symbentry sec_data_id sec_code_id dsz2 csz2 id (Some (Gvar v))) =
+      Some (get_symbentry sec_data_id sec_code_id dsz1 csz1 id def).
+Proof.
+  intros until csz2.
+  intros INT LINK.
+  destruct def1 as [def1|].
+  - inv LINK.
+    destr_in H0; try congruence. inv H0.
+    destruct def1; try (cbn in *; congruence).
+    simpl in Heqo. destr_in Heqo; try congruence.
+    inv Heqo.
+    unfold link_vardef in Heqo0.
+    repeat (destr_in Heqo0; try congruence).
+    cbn in Heqo1.
+    apply link_get_symbentry_right_extvar_init_comm; auto.
+  - inv LINK. 
+    unfold link_symb.   
+    rewrite get_var_entry_type.
+    rewrite get_none_entry_type.
+    replace (link_symbtype symb_notype symb_data) with (Some symb_data) by auto.
+    rewrite get_none_entry_secindex.
+    rewrite var_not_internal_iff in INT. 
+    destruct INT as [INT|INT].
+    + rewrite get_comm_var_entry_secindex; auto.
+      f_equal.
+      apply get_extern_symbentry_ignore_size.
+      cbn. rewrite var_not_internal_iff. auto.
+    + rewrite get_extern_var_entry_secindex; auto.
+      f_equal.
+      generalize (extern_var_init_nil v INT).
+      intros IL. 
+      cbn. rewrite IL. 
+      unfold update_symbtype. cbn. auto.
+Qed.
+
+Lemma link_get_symbentry_comm: forall def1 def2 def id dsz1 dsz2 csz1 csz2,
+    is_def_internal is_fundef_internal def2 = false ->
+    link_option def1 def2 = Some def 
+    -> link_symb (get_symbentry sec_data_id sec_code_id dsz1 csz1 id def1)
+                (get_symbentry sec_data_id sec_code_id dsz2 csz2 id def2) = 
+      Some (get_symbentry sec_data_id sec_code_id dsz1 csz1 id def).
+Proof.
+  intros until csz2.
+  intros INT LINK.
+  destruct def2 as [def2|].
+  - cbn in INT. destruct def2.
+    + apply link_getsymbentry_right_extfun; auto.
+    + apply link_getsymbentry_right_extvar; auto.
+  - apply link_get_symbentry_right_none_comm. auto.
+Qed.
+
+
+Lemma link_none_update_code_data_size: forall def1 def dsz1 csz1,
+    link_option def1 None = Some def
+    -> update_code_data_size dsz1 csz1 def1 = update_code_data_size dsz1 csz1 def.
+Proof.
+  intros until csz1.
+  intros LINK.
+  unfold link_option in LINK.
+  destruct def1 as [def1|].
+  - inv LINK. auto.
+  - inv LINK. auto.
+Qed.
+
+Lemma link_update_size_extvars_init_comm :
+  forall v1 (v2:globvar unit) dsz1 csz1 (inf:unit) init rd vl,
+    is_var_internal v1 = false 
+    -> is_var_internal v2 = false 
+    -> link_varinit (gvar_init v1) (gvar_init v2) = Some init
+    -> update_code_data_size dsz1 csz1 (Some (Gvar v1)) =
+      update_code_data_size dsz1 csz1
+                            (Some (Gvar (mkglobvar inf init rd vl))).
+Proof.
+  intros until vl.
+  intros INT1 INT2 LINK.
+  rewrite update_code_data_size_external_ignore_size; auto.
+  rewrite update_code_data_size_external_ignore_size; auto.
+  cbn.
+  generalize (link_external_varinit _ _ _ INT1 INT2 LINK).
+  intros.
+  unfold is_var_internal. cbn.
+  destruct (classify_init init); congruence.
+Qed.    
+
+
+Lemma link_update_size_right_extvar_init_comm :
+  forall v1 (v2: globvar unit) dsz1 csz1 (inf:unit) init rd vl,
+    is_var_internal v2 = false 
+    -> link_varinit (gvar_init v1) (gvar_init v2) = Some init
+    -> update_code_data_size dsz1 csz1 (Some (Gvar v1)) =
+      update_code_data_size dsz1 csz1 (Some (Gvar (mkglobvar inf init rd vl))).
+Proof.
+  intros until vl.
+  intros INT LINK.
+  destruct (is_var_internal v1) eqn:INT1.
+  generalize INT. intros INT'.
+  rewrite var_not_internal_iff in INT.
+  destruct INT as [INT|INT].
+  - generalize (link_internal_comm_varinit _ _ _ INT1 INT LINK).
+    destruct 1 as (IEQ & SEQ & CLS1). subst.
+    auto.
+  - generalize (link_internal_external_varinit _ _ _ INT1 INT' LINK).
+    destruct 1 as (INITEQ & CLS). subst.
+    auto.
+  - apply link_update_size_extvars_init_comm with v2; auto.
+Qed.
+
+
+Lemma link_extern_vardef_update_code_data_size: forall def1 v def dsz1 csz1,
+        is_var_internal v = false
+        -> link_option def1 (Some (Gvar v)) = Some def
+        -> update_code_data_size dsz1 csz1 def1 = update_code_data_size dsz1 csz1 def.
+Proof.
+  intros until csz1.
+  intros INT LINK.
+  destruct def1 as [def1|].
+  - cbn in LINK.
+    destr_in LINK; try congruence. inv LINK.
+    destruct def1; try (cbn in *; congruence).
+    simpl in Heqo. destr_in Heqo; try congruence.
+    inv Heqo.
+    unfold link_vardef in Heqo0.
+    repeat (destr_in Heqo0; try congruence).
+    cbn in Heqo1.
+    apply link_update_size_right_extvar_init_comm with v; auto.
+  - cbn in LINK. inv LINK.
+    rewrite (update_code_data_size_external_ignore_size (Some (Gvar v))).
+    simpl. auto.
+    cbn. auto.
+Qed.
+  
+Lemma link_update_size_right_extfun_comm :
+  forall f1 f2 f dsz1 csz1,
+    is_fundef_internal f2 = false 
+    -> link_fundef f1 f2 = Some f
+    -> update_code_data_size dsz1 csz1 (Some (Gfun f1)) =
+       update_code_data_size dsz1 csz1 (Some (Gfun f)).
+Proof.
+  intros until csz1.
+  intros INT LINK.
+  destruct f2; try (cbn in INT; congruence).
+  apply link_fundef_inv1 in LINK. subst.
+  auto.
+Qed.
+  
+
+Lemma link_extern_fundef_update_code_data_size: forall def1 f def dsz1 csz1,
+        is_fundef_internal f = false
+        -> link_option def1 (Some (Gfun f)) = Some def
+        -> update_code_data_size dsz1 csz1 def1 = update_code_data_size dsz1 csz1 def.
+Proof.
+  intros until csz1.
+  intros INT LINK.
+  destruct def1 as [def1|].
+  - cbn in LINK.
+    destr_in LINK; try congruence. inv LINK.
+    destruct def1; try (cbn in *; congruence).
+    simpl in Heqo. destr_in Heqo; try congruence.
+    inv Heqo.
+    apply link_update_size_right_extfun_comm with f; auto.    
+  - cbn in LINK.  inv LINK.
+    rewrite (update_code_data_size_external_ignore_size (Some (Gfun f))).
+    simpl. auto.
+    cbn. auto.
+Qed.
+
+
+Lemma link_extern_def_update_code_data_size: forall def1 def2 def dsz1 csz1,
+    is_def_internal is_fundef_internal def2 = false
+    -> link_option def1 def2 = Some def
+    -> update_code_data_size dsz1 csz1 def1 = update_code_data_size dsz1 csz1 def.
+Proof.
+  intros until csz1.
+  intros INT LINK.
+  destruct def2 as [def2|].
+  - cbn in INT. destruct def2.
+    + apply link_extern_fundef_update_code_data_size with f; auto.
+    + apply link_extern_vardef_update_code_data_size with v; auto.
+  - apply link_none_update_code_data_size. auto.
+Qed.
+
+
+(* Lemma link_defs1_acc_symb_comm : forall asf defs1 defs2 defs1_linked defs1_rest defs2_rest rstbl1 rstbl2 dsz1 dsz2 csz1 csz2 dsz1' csz1', *)
+(*     asf = acc_symb sec_data_id sec_code_id -> *)
+(*     list_norepet (map fst defs2) -> *)
+(*     link_defs1 is_fundef_internal defs1 defs2 = Some (defs1_linked, defs1_rest, defs2_rest) -> *)
+(*     fold_left asf defs1 ([], dsz1', csz1') = (rstbl1, dsz1, csz1) -> *)
+(*     fold_left asf defs2 ([], 0, 0) = (rstbl2, dsz2, csz2) -> *)
+(*     exists rstbl1_linked rstbl1_rest rstbl2_rest, *)
+(*       link_symbtable1 (rev rstbl1) (rev rstbl2) = Some (rev rstbl1_linked, rev rstbl1_rest, rev rstbl2_rest) /\ *)
+(*       fold_left asf defs1_linked ([], dsz1', csz1') = (rstbl1_linked, dsz1, csz1) /\ *)
+(*       fold_left asf defs1_rest ([], 0, 0) = (rstbl1_rest, 0, 0) /\ *)
+(*       fold_left asf defs2_rest ([], 0, 0) = (rstbl2_rest, dsz2, csz2). *)
+(* Proof. *)
+(*   induction defs1 as [|def1 defs1]. *)
+(*   - intros until csz1'. *)
+(*     intros ASF NORPT LINK ACC1 ACC2. *)
+(*     simpl in *. inv ACC1. inv LINK. simpl. *)
+(*     repeat eexists; auto. *)
+(*   - intros until csz1'. *)
+(*     intros ASF NORPT LINK ACC1 ACC2.  *)
+(*     simpl in *. destruct def1 as (id1 & def1). *)
+(*     destruct (link_defs1 is_fundef_internal defs1 defs2) as [r|] eqn:LINK_TAIL; *)
+(*       try congruence. *)
+(*     destruct r as (p & defs2_rest').  *)
+(*     destruct p as (defs1_linked' & defs1_rest'). *)
+(*     rewrite ASF in ACC1. simpl in ACC1. *)
+(*     destruct (update_code_data_size dsz1' csz1' def1) as (dsz1'' & csz1'') eqn:UPDATE. *)
+    
+(*     rewrite <- ASF in ACC1. *)
+(*     generalize (acc_symb_inv _ _ _ _ ASF ACC1). *)
+(*     destruct 1 as (stbl1' & STEQ & ACC1'). *)
+(*     generalize (IHdefs1 _ _ _ _ _ _ _ _ _ _ _ _ ASF NORPT LINK_TAIL ACC1' ACC2). *)
+(*     destruct 1 as (stbl1_linked & stbl1_rest & stbl2_rest & LINK_SYMB_TAIL & ACC_LINK1 & ACC_REST1 & ACC_REST2). *)
+    
+(*     destruct (partition (fun '(id', _) => ident_eq id' id1) defs2_rest') as (defs2' & defs2_rest'') eqn:PART. *)
+(*     subst rstbl1. rewrite rev_unit. *)
+(*     simpl. rewrite LINK_SYMB_TAIL. *)
+(*     rewrite get_symbentry_id. *)
+
+(*     destruct defs2' as [|defs2']. *)
+(*     + (* No definition with id1 was found in the second module *) *)
+(*       generalize (partition_inv_nil1 _ _ PART). intros. subst defs2_rest''. *)
+(*       inversion LINK.  *)
+(*       subst defs1_linked. subst defs1_rest. subst defs2_rest. *)
+(*       generalize (acc_symb_pres_partition _ _ _ _ ASF PART ACC_REST2). *)
+(*       destruct 1 as (stbl1 & stbl2 & PART' & MATCH1 & MATCH2). *)
+(*       inversion MATCH1; clear MATCH1. subst stbl1. *)
+(*       generalize (partition_inv_nil1 _ _ PART'). intros. subst stbl2. *)
+(*       rewrite PART'. *)
+(*       rewrite <- rev_unit.  *)
+(*       do 3 eexists. split. auto. *)
+(*       split; auto. subst asf. simpl. rewrite UPDATE. *)
+(*       apply acc_symb_append_nil. auto. *)
+      
+(*     + (* Some definition with id1 was found in the second module *) *)
+(*       destruct defs2' as (id, def2). *)
+(*       destruct (is_def_internal is_fundef_internal def2) eqn:DEF2_INT. *)
+(*       * (* The found definition is internal *) *)
+(*         destruct (is_def_internal is_fundef_internal def1) eqn:DEF1_INT; try congruence. *)
+(*         inversion LINK; clear LINK. *)
+(*         subst defs1_linked'. subst defs1_rest. subst defs2_rest'. *)
+(*         generalize (acc_symb_pres_partition _ _ _ _ ASF PART ACC_REST2). *)
+(*         destruct 1 as (stbl1 & stbl2 & PART' & MATCH1 & MATCH2). *)
+(*         rewrite PART'. inv MATCH1.                 *)
+(*         erewrite <- match_def_symbentry_pres_internal_prop; eauto. *)
+(*         rewrite DEF2_INT. *)
+(*         erewrite <- get_symbentry_pres_internal_prop; eauto. *)
+(*         rewrite DEF1_INT. *)
+(*         rewrite <- rev_unit. *)
+(*         do 3 eexists. split; auto. *)
+(*         split; auto. *)
+(*         generalize (update_code_data_size_external_size_inv _ _ _ DEF1_INT UPDATE). *)
+(*         destruct 1. subst. auto. *)
+(*         split; auto. *)
+(*         simpl. destr. *)
+(*         generalize (update_code_data_size_external_size_inv _ _ _ DEF1_INT Heqp). *)
+(*         destruct 1. subst. *)
+(*         rewrite (get_extern_symbentry_ignore_size id1 def1 0 0 dsz1' csz1'); auto. *)
+(*         apply acc_symb_append_nil. auto. *)
+
+(*       * (* The found definition is external *) *)
+(*         destruct (link_option def1 def2) as [def|] eqn:LINKDEF; try congruence. *)
+(*         assert (defs2'0 = nil). *)
+(*         {  *)
+(*           generalize (link_defs_rest_norepet_pres2 _ _ _ _ NORPT LINK_TAIL). *)
+(*           intros NORPT'. *)
+(*           generalize (lst_norepet_partition_inv _ _ NORPT' PART). *)
+(*           destruct 1 as [ DEQ | DEQ ]; try congruence. *)
+(*           destruct DEQ as (def2' & DEQ). *)
+(*           inv DEQ. auto. *)
+(*         }   *)
+(*         subst defs2'0. *)
+(*         assert (Forall (fun '(_, def) => is_def_internal is_fundef_internal def = false) [(id, def2)]) as DEF2INT'. *)
+(*         { constructor. auto. apply Forall_nil. } *)
+(*         generalize (acc_symb_partition_extern_intern _ _ _ _ ASF PART ACC_REST2 DEF2INT'). *)
+(*         destruct 1 as (stbl2' & stbl2_rest' & PART' & ACC2_REST' & ACC2_REST''). *)
+(*         inversion LINK. subst defs1_linked. subst defs1_rest'. subst defs2_rest''. *)
+(*         rewrite PART'.  *)
+(*         rewrite ASF in ACC2_REST'; simpl in ACC2_REST'. *)
+(*         rewrite (update_code_data_size_external_ignore_size def2 0 0) in ACC2_REST'; auto. *)
+(*         inversion ACC2_REST'.            *)
+(*         symmetry in H0. apply rev_single in H0. subst stbl2'. *)
+(*         rewrite <- get_symbentry_pres_internal_prop. rewrite DEF2_INT. *)
+(*         (* rewrite DEF2_INT. red in H1. destruct H1 as (dsz & csz & EQ). *) *)
+(*         (* subst y.         *) *)
+(*         generalize (elements_in_partition_prop _ _ PART'). *)
+(*         destruct 1 as (ELEM1 & ELEM2). *)
+(*         generalize (ELEM1 _ (in_eq _ _)). *)
+(*         unfold symbentry_id_eq. rewrite get_symbentry_id. *)
+(*         intros IDEQ. destruct ident_eq; try congruence. subst id1. *)
+(*         generalize (link_get_symbentry_comm _ _ id dsz1' 0 csz1' 0 DEF2_INT LINKDEF). *)
+(*         intros LINKSYMB. *)
+(*         rewrite LINKSYMB. *)
+(*         rewrite <- rev_unit. rewrite <- (rev_involutive stbl2_rest'). *)
+(*         do 3 eexists; split; auto. *)
+(*         split; auto. *)
+(*         rewrite ASF. simpl. *)
+(*         erewrite <- link_extern_def_update_code_data_size; eauto. *)
+(*         rewrite UPDATE. *)
+(*         apply acc_symb_append_nil. rewrite ASF in ACC_LINK1. auto. *)
+(* Qed. *)
+        
+
+(* Lemma link_defs1_gen_symbtbl_comm : forall defs1 defs2 defs1_linked defs1_rest defs2_rest stbl1 stbl2 dsz1 dsz2 csz1 csz2, *)
+(*     list_norepet (map fst defs2) -> *)
+(*     link_defs1 is_fundef_internal defs1 defs2 = Some (defs1_linked, defs1_rest, defs2_rest) -> *)
+(*     gen_symb_table sec_data_id sec_code_id defs1 = (stbl1, dsz1, csz1) -> *)
+(*     gen_symb_table sec_data_id sec_code_id defs2 = (stbl2, dsz2, csz2) -> *)
+(*     exists stbl1_linked stbl1_rest stbl2_rest, *)
+(*       link_symbtable1 stbl1 stbl2 = Some (stbl1_linked, stbl1_rest, stbl2_rest) /\ *)
+(*       gen_symb_table sec_data_id sec_code_id defs1_linked = (stbl1_linked, dsz1, csz1) /\ *)
+(*       gen_symb_table sec_data_id sec_code_id defs1_rest = (stbl1_rest, 0, 0) /\ *)
+(*       gen_symb_table sec_data_id sec_code_id defs2_rest = (stbl2_rest, dsz2, csz2). *)
+(* Proof. *)
+(*   intros until csz2.  *)
+(*   intros NORPT LINK GS1 GS2. unfold gen_symb_table in GS1, GS2. *)
+(*   destr_in GS1. destruct p. inv GS1. *)
+(*   destr_in GS2. destruct p. inv GS2. *)
+(*   generalize (link_defs1_acc_symb_comm _ _ _ _ (@eq_refl _ (acc_symb sec_data_id sec_code_id)) NORPT LINK Heqp Heqp0). *)
+(*   destruct 1 as (t1 & t1' & t2 & LINKS & GS1 & GS2 & GS3). *)
+(*   unfold gen_symb_table. *)
+(*   rewrite LINKS, GS1, GS2, GS3.  *)
+(*   repeat eexists; eauto. *)
+(* Qed. *)
+
+Lemma partition_reloc_symbtable_comm : forall f l l1 l2 rf l',
+    (forall e e', reloc_symb rf e = Some e' -> f e = f e') 
+    -> partition f l = (l1, l2)
+    -> reloc_symbtable rf l = Some l'
+    -> exists l1' l2', partition f l' = (l1', l2') 
+                 /\ reloc_symbtable rf l1 = Some l1'
+                 /\ reloc_symbtable rf l2 = Some l2'.
+Proof.
+  induction l as [| e l].
+  - intros l1 l2 rf l' PRES PART RELOC.
+    cbn in *. inv PART. inv RELOC.
+    exists nil, nil.
+    split; auto.
+  - intros l1 l2 rf l' PRES PART RELOC.
+    cbn in *. destr_in PART. destruct (f e) eqn:PEQ.
+    + inv PART.
+      unfold reloc_iter in RELOC. 
+      destr_in RELOC; try congruence.
+      destr_in RELOC; try congruence.
+      inv RELOC.
+      generalize (IHl _ _ _ _ PRES eq_refl Heqo).
+      destruct 1 as (l1' & l2' & PART' & RELOC1 & RELOC2).
+      exists (s :: l1'), l2'. 
+      erewrite PRES in PEQ; eauto.
+      cbn. rewrite PEQ. rewrite PART'.
+      split; auto.
+      split; auto.
+      unfold reloc_iter. setoid_rewrite RELOC1.
+      rewrite Heqo0. auto.
+    + inv PART.
+      unfold reloc_iter in RELOC. 
+      destr_in RELOC; try congruence.
+      destr_in RELOC; try congruence.
+      inv RELOC.
+      generalize (IHl _ _ _ _ PRES eq_refl Heqo).
+      destruct 1 as (l1' & l2' & PART' & RELOC1 & RELOC2).
+      exists (l1'), (s ::l2'). 
+      erewrite PRES in PEQ; eauto.
+      cbn. rewrite PEQ. rewrite PART'.
+      split; auto.
+      split; auto.
+      unfold reloc_iter. setoid_rewrite RELOC2.
+      rewrite Heqo0. auto.
+Qed.    
+
+
+Lemma reloc_symb_pres_internal_prop : forall rf s1 s2,
+    reloc_symb rf s1 = Some s2 
+    -> is_symbentry_internal s1 = is_symbentry_internal s2.
+Proof.
+  intros rf s1 s2 RELOC.
+  unfold reloc_symb in RELOC. 
+  unfold is_symbentry_internal.
+  destr_in RELOC.
+  destr_in RELOC.
+  inv RELOC. cbn. auto.
+  inv RELOC. rewrite Heqs. auto.
+  inv RELOC. rewrite Heqs. auto.
+Qed.
+
+Lemma reloc_external_symb : forall rf s,
+    is_symbentry_internal s = false
+    -> reloc_symb rf s = Some s. 
+Proof.
+  intros rf s RELOC.
+  unfold is_symbentry_internal in RELOC.
+  unfold reloc_symb. destr_in RELOC.
+Qed.  
+
+Lemma reloc_symb_pres_id: forall rf e e', 
+      reloc_symb rf e = Some e' -> symbentry_id e = symbentry_id e'.
+Proof.
+  intros rf e e' RELOC.
+  unfold reloc_symb in RELOC.
+  destruct e. cbn in *.
+  destruct symbentry_secindex. destruct (rf idx).
+  inv RELOC. cbn. auto.
+  congruence.
+  inv RELOC. cbn. auto.
+  inv RELOC. cbn. auto.
+Qed.
+
+Lemma reloc_symb_pres_type: forall rf e e', 
+      reloc_symb rf e = Some e' -> symbentry_type e = symbentry_type e'.
+Proof.
+  intros rf e e' RELOC.
+  unfold reloc_symb in RELOC.
+  destruct e. cbn in *.
+  destruct symbentry_secindex. destruct (rf idx).
+  inv RELOC. cbn. auto.
+  congruence.
+  inv RELOC. cbn. auto.
+  inv RELOC. cbn. auto.
+Qed.
+
+Lemma reloc_symb_pres_secindex: forall rf e e', 
+      reloc_symb rf e = Some e' -> symbentry_secindex e = symbentry_secindex e'.
+Proof.
+  intros rf e e' RELOC.
+  unfold reloc_symb in RELOC.
+  destruct e. cbn in *.
+  destruct symbentry_secindex. destruct (rf idx).
+  inv RELOC. cbn. auto.
+  congruence.
+  inv RELOC. cbn. auto.
+  inv RELOC. cbn. auto.
+Qed.
+
+Lemma reloc_symb_pres_size: forall rf e e', 
+      reloc_symb rf e = Some e' -> symbentry_size e = symbentry_size e'.
+Proof.
+  intros rf e e' RELOC.
+  unfold reloc_symb in RELOC.
+  destruct e. cbn in *.
+  destruct symbentry_secindex. destruct (rf idx).
+  inv RELOC. cbn. auto.
+  congruence.
+  inv RELOC. cbn. auto.
+  inv RELOC. cbn. auto.
+Qed.
+
+Lemma reloc_symb_pres_update_symbtype : forall rf e e' t,
+    reloc_symb rf e = Some e' ->
+    reloc_symb rf (update_symbtype e t) = Some (update_symbtype e' t).
+Proof.
+  intros rf e e' t RELOC.
+  destruct e. unfold reloc_symb in *. cbn in *.
+  destr_in RELOC; try congruence; subst.
+  destr_in RELOC; try congruence.
+  inv RELOC. auto.
+Qed.
+
+
+
+Lemma reloc_symb_id_eq: forall id rf e e', 
+      reloc_symb rf e = Some e' -> symbentry_id_eq id e = symbentry_id_eq id e'.
+Proof.
+  intros.
+  unfold symbentry_id_eq.
+  erewrite reloc_symb_pres_id; eauto.
+Qed.
+
+(* Lemma reloc_link_symbtable_comm2: forall rf stbl1 stbl2 stbl2' stbl1_linked stbl1_rest stbl2_rest, *)
+(*     reloc_symbtable rf stbl2 = Some stbl2' -> *)
+(*     link_symbtable1 stbl1 stbl2 = Some (stbl1_linked, stbl1_rest, stbl2_rest) -> *)
+(*     exists stbl2_rest', reloc_symbtable rf stbl2_rest = Some stbl2_rest' /\ *)
+(*                    link_symbtable1 stbl1 stbl2' = Some (stbl1_linked, stbl1_rest, stbl2_rest'). *)
+(* Proof. *)
+(*   induction stbl1 as [|e stbl1]. *)
+(*   - intros until stbl2_rest. *)
+(*     intros RELOC LINK. cbn in *. inv LINK. *)
+(*     eauto. *)
+(*   - intros until stbl2_rest. *)
+(*     intros RELOC LINK. cbn in *. *)
+(*     destr_in LINK; try congruence. destruct p. destruct p. *)
+(*     destr_in LINK; try congruence. destr_in LINK.  *)
+(*     generalize (IHstbl1 _ _ _ _ _ RELOC Heqo). *)
+(*     destruct 1 as (stbl2_rest' & RELOC' & LINK'). *)
+(*     destruct l. *)
+(*     + inv LINK. generalize (partition_inv_nil1 _ _ Heqp). intros. subst l0. *)
+(*       exists stbl2_rest'; split; auto. *)
+(*       rewrite LINK'.       *)
+(*       generalize (partition_reloc_symbtable_comm _ _ _ (reloc_symb_id_eq i rf) Heqp RELOC'). *)
+(*       destruct 1 as (l1' & l2' & PART & RELOC1 & RELOC2). *)
+(*       cbn in RELOC1. inv RELOC1. *)
+(*       generalize (partition_inv_nil1 _ _ PART). intros. subst l2'. *)
+(*       rewrite PART. auto. *)
+(*     + destr_in LINK. *)
+(*       * destr_in LINK; try congruence. *)
+(*         inv LINK. *)
+(*         exists stbl2_rest'. split; auto. *)
+(*         rewrite LINK'.  *)
+(*         generalize (partition_reloc_symbtable_comm _ _ _ (reloc_symb_id_eq i rf) Heqp RELOC'). *)
+(*         destruct 1 as (l1' & l2' & PART & RELOC1 & RELOC2). *)
+(*         rewrite PART. cbn in RELOC1. *)
+(*         unfold reloc_iter in RELOC1. *)
+(*         destr_in RELOC1; try congruence. *)
+(*         destr_in RELOC1; try congruence. *)
+(*         inv RELOC1. *)
+(*         erewrite <- reloc_symb_pres_internal_prop; eauto. *)
+(*         rewrite Heqb. auto. *)
+(*       * destr_in LINK; try congruence. *)
+(*         inv LINK. *)
+(*         rewrite LINK'. *)
+(*         generalize (partition_reloc_symbtable_comm _ _ _ (reloc_symb_id_eq i rf) Heqp RELOC'). *)
+(*         destruct 1 as (l1' & l2' & PART & RELOC1 & RELOC2). *)
+(*         rewrite RELOC2. eexists; split; eauto. *)
+(*         rewrite PART. *)
+(*         cbn in RELOC1. unfold reloc_iter in RELOC1. *)
+(*         destr_in RELOC1; try congruence. *)
+(*         destr_in RELOC1; try congruence. inv RELOC1. *)
+(*         erewrite <- reloc_symb_pres_internal_prop; eauto. *)
+(*         rewrite Heqb.          *)
+(*         erewrite reloc_external_symb in Heqo3; eauto. inv Heqo3. *)
+(*         rewrite Heqo1. auto. *)
+(* Qed. *)
+  
+
+(* Lemma reloc_link_symb_comm : forall e1 e2 e e1' rf, *)
+(*     is_symbentry_internal e2 = false  *)
+(*     -> reloc_symb rf e1 = Some e1' *)
+(*     -> link_symb e1 e2 = Some e *)
+(*     -> exists e', reloc_symb rf e = Some e' /\ link_symb e1' e2 = Some e'. *)
+(* Proof. *)
+(*   intros e1 e2 e e1' rf INT RELOC LINK. *)
+(*   unfold link_symb in *. *)
+(*   erewrite <- reloc_symb_pres_type; eauto. *)
+(*   erewrite <- reloc_symb_pres_secindex; eauto. *)
+(*   erewrite <- reloc_symb_pres_size; eauto. *)
+(*   destr_in LINK; try congruence. *)
+(*   destr_in LINK. *)
+(*   - destr_in LINK; try congruence. *)
+(*     + destruct zeq; try congruence. inv LINK. *)
+(*       rewrite RELOC. eexists; split; eauto. *)
+(*     + inv LINK. eauto. *)
+(*   - destr_in LINK; try congruence. *)
+(*     + destruct zeq; try congruence. inv LINK. *)
+(*       exists e; split; auto. *)
+(*       apply reloc_external_symb; auto. *)
+(*     + destruct zeq; try congruence. inv LINK. *)
+(*       rewrite RELOC. eexists; split; eauto.  *)
+(*     + inv LINK. rewrite RELOC. eexists; split; eauto.  *)
+(*   - destr_in LINK; try congruence. *)
+(*     + inv LINK. *)
+(*       exists e; split; auto. *)
+(*       apply reloc_external_symb; auto. *)
+(*     + inv LINK. exists e; split; auto. *)
+(*       apply reloc_external_symb; auto. *)
+(*     + inv LINK.  *)
+(*       eexists; split; eauto.      *)
+(*       apply reloc_symb_pres_update_symbtype; auto. *)
+(* Qed. *)
+
+
+(* Lemma reloc_link_symbtable_comm1: forall rf stbl1 stbl2 stbl1' stbl1_linked stbl1_rest stbl2_rest, *)
+(*     reloc_symbtable rf stbl1 = Some stbl1' -> *)
+(*     link_symbtable1 stbl1 stbl2 = Some (stbl1_linked, stbl1_rest, stbl2_rest) -> *)
+(*     exists stbl1_linked', reloc_symbtable rf stbl1_linked = Some stbl1_linked' /\ *)
+(*                      link_symbtable1 stbl1' stbl2 = Some (stbl1_linked', stbl1_rest, stbl2_rest). *)
+(* Proof. *)
+(*     induction stbl1 as [|e stbl1]. *)
+(*   - intros until stbl2_rest. *)
+(*     intros RELOC LINK. cbn in *. inv RELOC. inv LINK. *)
+(*     exists nil. split; auto. *)
+(*   - intros until stbl2_rest. *)
+(*     intros RELOC LINK. cbn in *. *)
+(*     unfold reloc_iter in RELOC. *)
+(*     destr_in RELOC; try congruence. *)
+(*     destr_in RELOC; try congruence. inv RELOC. *)
+(*     destr_in LINK; try congruence. destruct p. destruct p. *)
+(*     destr_in LINK; try congruence. destr_in LINK.  *)
+(*     generalize (IHstbl1 _ _ _ _ _ Heqo Heqo1). *)
+(*     destruct 1 as (stbl1_rest' & RELOC' & LINK'). *)
+(*     destruct l0. *)
+(*     + inv LINK. generalize (partition_inv_nil1 _ _ Heqp). intros. subst l1. *)
+(*       exists (s :: stbl1_rest'); split; auto. *)
+(*       cbn. unfold reloc_iter. *)
+(*       setoid_rewrite RELOC'. rewrite Heqo0. auto. *)
+(*       cbn. rewrite LINK'.  *)
+(*       erewrite <- reloc_symb_pres_id; eauto. rewrite Heqo2. *)
+(*       rewrite Heqp. auto. *)
+(*     + destr_in LINK. *)
+(*       * destr_in LINK; try congruence. *)
+(*         inv LINK. *)
+(*         exists stbl1_rest'. split; auto. *)
+(*         cbn. *)
+(*         rewrite LINK'.  *)
+(*         erewrite <- reloc_symb_pres_id; eauto. rewrite Heqo2. *)
+(*         rewrite Heqp. rewrite Heqb.  *)
+(*         erewrite <- reloc_symb_pres_internal_prop; eauto. rewrite Heqb0. *)
+(*         erewrite reloc_external_symb in Heqo0; eauto. inv Heqo0. *)
+(*         auto. *)
+(*       * destr_in LINK; try congruence. *)
+(*         inv LINK. *)
+(*         generalize (reloc_link_symb_comm _ _ _ Heqb Heqo0 Heqo3). *)
+(*         destruct 1 as (e' & RELOCS & LINKS). *)
+(*         exists (e' :: stbl1_rest'). split. *)
+(*         ** cbn. unfold reloc_iter. *)
+(*            setoid_rewrite RELOC'. rewrite RELOCS. auto. *)
+(*         ** cbn. *)
+(*            rewrite LINK'.  *)
+(*            erewrite <- reloc_symb_pres_id; eauto. rewrite Heqo2. *)
+(*            rewrite Heqp. rewrite Heqb. rewrite LINKS. *)
+(*            auto. *)
+(* Qed. *)
+
+Lemma update_size_offset : forall def dsz csz dsz1 csz1 dofs cofs,
+    update_code_data_size dsz csz def = (dsz1, csz1) ->
+    update_code_data_size (dofs + dsz) (cofs + csz) def = (dofs + dsz1, cofs + csz1).
+Proof.
+  intros until cofs. intros UPDATE.
+  destruct def. destruct g. destruct f.
+  - cbn in *. inv UPDATE. f_equal; omega.
+  - cbn in *. inv UPDATE. f_equal; omega.
+  - unfold update_code_data_size in *.
+    destr_in UPDATE. 
+    destruct i; try (inv UPDATE; cbn; f_equal; omega).
+    destruct l; try (inv UPDATE; cbn; f_equal; omega).
+  - cbn in *. inv UPDATE. auto.
+Qed.
+
+Lemma reloc_get_symbentry : forall dofs cofs dsz csz id def e,
+    reloc_symb (reloc_offset_fun dofs cofs) (get_symbentry sec_data_id sec_code_id dsz csz id def) = Some e
+    -> e = (get_symbentry sec_data_id sec_code_id (dsz + dofs) (csz + cofs) id def).
+Proof.
+  intros until e. intro RELOC.
+  destruct def. destruct g. destruct f.
+  - cbn in *. inv RELOC. f_equal.
+  - cbn in *. inv RELOC. auto.
+  - cbn in *. destr_in RELOC. cbn in *. inv RELOC. auto.
+    destruct i; cbn in *; try congruence.
+    destruct l; cbn in *; try congruence.
+  - cbn in *. inv RELOC. auto.
+Qed.
+
+Lemma acc_symb_reloc: forall asf defs stbl stbl' dsz1 dsz2 csz1 csz2 dofs cofs,
+    asf = (acc_symb sec_data_id sec_code_id) 
+    -> fold_left asf defs ([], dsz1, csz1) = (stbl, dsz2, csz2)
+    -> reloc_symbtable (reloc_offset_fun dofs cofs) (rev stbl) = Some stbl'
+    -> fold_left asf defs ([], dofs + dsz1, cofs + csz1) = (rev stbl', dofs + dsz2, cofs + csz2).
+Proof.
+  induction defs as [|def defs].
+  - intros until cofs. intros ASF ACC RELOC.
+    cbn in *. inv ACC. cbn in RELOC. inv RELOC. auto.
+  - intros until cofs. intros ASF ACC RELOC.
+    subst. cbn in *. destruct def as [id def].
+    destr_in ACC.
+    generalize (acc_symb_inv _ _ _ _ eq_refl ACC).
+    destruct 1 as (stbl1 & EQ & ACC1). subst.    
+    erewrite update_size_offset; eauto.
+    rewrite rev_unit in RELOC.
+    cbn in RELOC. unfold reloc_iter in RELOC.
+    destr_in RELOC; try congruence.
+    destr_in RELOC; try congruence.
+    inv RELOC.
+    generalize (IHdefs _ _ _ _ _ _ _ _ eq_refl ACC1 Heqo).
+    intros ACC'.
+    generalize (acc_symb_append_nil _ _ _ _ _ 
+                                    [get_symbentry sec_data_id sec_code_id (dofs + dsz1) (cofs + csz1) id def] ACC').
+    intros ACC''. setoid_rewrite ACC''.
+    cbn. f_equal. f_equal.
+    apply reloc_get_symbentry in Heqo0. subst. 
+    f_equal. f_equal. f_equal; omega.
+Qed.    
+
+
+Lemma acc_symb_reloc_comm: forall asf defs1 defs2 stbl1 stbl2 stbl2'
+                             dsz1 dsz2 csz1 csz2 dsz1' csz1',
+    asf = (acc_symb sec_data_id sec_code_id) 
+    -> fold_left asf defs1 ([], dsz1, csz1) = (stbl1, dsz1', csz1')
+    -> fold_left asf defs2 ([], 0, 0) = (stbl2, dsz2, csz2)
+    -> reloc_symbtable (reloc_offset_fun dsz1' csz1') (rev stbl2) = Some stbl2'
+    -> fold_left asf (defs1 ++ defs2) ([], dsz1, csz1) = ((rev stbl2') ++ stbl1, dsz1' + dsz2, csz1' + csz2).
+Proof.
+  induction defs1.
+  - intros until csz1'.
+    intros ASF ACC1 ACC2 RELOC.
+    cbn in *. inv ACC1.
+    rewrite app_nil_r.
+    replace ([], dsz1', csz1') with (@nil symbentry, dsz1'+0, csz1'+0).
+    eapply acc_symb_reloc; eauto.
+    f_equal. f_equal. omega. omega.
+  - intros until csz1'.
+    intros ASF ACC1 ACC2 RELOC.
+    cbn in *. rewrite ASF in ACC1. unfold acc_symb in ACC1.
+    destruct a as [id def]. destr_in ACC1.
+    generalize (acc_symb_inv _ _ _ _ eq_refl ACC1).
+    destruct 1 as (stbl1' & SEQ & ACC1'). subst.
+    generalize (IHdefs1 _ _ _ _ _ _ _ _ _ _ eq_refl ACC1' ACC2 RELOC).
+    intros ACC'.
+    unfold acc_symb. rewrite Heqp. 
+    setoid_rewrite acc_symb_append_nil; eauto.
+    rewrite app_assoc. auto.
+Qed.
+  
+
+Lemma gen_symb_table_reloc_comm : forall defs1 defs2 stbl1 stbl2 stbl2' dsz1 dsz2 csz1 csz2,
+    gen_symb_table sec_data_id sec_code_id defs1 = (stbl1, dsz1, csz1) ->
+    gen_symb_table sec_data_id sec_code_id defs2 = (stbl2, dsz2, csz2) ->
+    reloc_symbtable (reloc_offset_fun dsz1 csz1) stbl2 = Some stbl2' ->
+    gen_symb_table sec_data_id sec_code_id (defs1 ++ defs2) = (stbl1 ++ stbl2', dsz1 + dsz2, csz1 + csz2).
+Proof.
+  intros until csz2.
+  intros GS1 GS2 RELOC.
+  unfold gen_symb_table in GS1, GS2.
+  destr_in GS1; inv GS1.
+  destr_in GS2; inv GS2.
+  destruct p, p0. inv H0. inv H1.
+  unfold gen_symb_table.  
+Admitted.
+(*   erewrite acc_symb_reloc_comm; eauto. *)
+(*   rewrite rev_app_distr. rewrite rev_involutive. *)
+(*   auto. *)
+(* Qed. *)
+
+
+(* Lemma link_gen_symb_comm : forall defs1 defs2 defs stbl1 stbl2 dsz1 csz1 dsz2 csz2 f_ofs, *)
+(*     list_norepet (map fst defs1) -> *)
+(*     list_norepet (map fst defs2) -> *)
+(*     link_defs is_fundef_internal defs1 defs2 = Some defs -> *)
+(*     gen_symb_table sec_data_id sec_code_id defs1 = (stbl1, dsz1, csz1) -> *)
+(*     gen_symb_table sec_data_id sec_code_id defs2 = (stbl2, dsz2, csz2) -> *)
+(*     f_ofs = reloc_offset_fun dsz1 csz1 -> *)
+(*     exists stbl stbl2', *)
+(*       reloc_symbtable f_ofs stbl2 = Some stbl2' /\ *)
+(*       link_symbtable stbl1 stbl2' = Some stbl *)
+(*       /\ gen_symb_table sec_data_id sec_code_id defs = (stbl, dsz1 + dsz2, csz1 + csz2). *)
+(* Proof. *)
+(*   intros defs1 defs2 defs stbl1 stbl2 dsz1 csz1 dsz2 csz2 f_ofs NORPT1 NORPT2 LINK GS1 GS2 FOFS. *)
+
+(*   unfold link_defs in LINK. *)
+(*   destruct (link_defs1 is_fundef_internal defs1 defs2) as [r|] eqn:LINKDEFS1;  *)
+(*     try congruence. *)
+(*   destruct r as (p & defs2_rest). destruct p as (defs1_linked, defs1_rest). *)
+(*   destruct (link_defs1 is_fundef_internal defs2_rest defs1_rest) as [r|] eqn:LINKDEFS2;  *)
+(*     try congruence. *)
+(*   destruct r. destruct p as (defs2_linked & r). inv LINK. *)
+
+(*   generalize (link_defs1_gen_symbtbl_comm _ _ NORPT2 LINKDEFS1 GS1 GS2). *)
+(*   destruct 1 as (stbl1_linked & stlb1_rest & stbl2_rest & LINKSTBL1 & GSLINKED1 & GSREST1 & GSREST2). *)
+(*   generalize (reloc_symbtable_exists _ GS2 (@eq_refl _ (reloc_offset_fun dsz1 csz1))). *)
+(*   destruct 1 as (stbl2' & RELOC & RELOC_PROP). *)
+(*   generalize (reloc_link_symbtable_comm2 _ _ _ RELOC LINKSTBL1). *)
+(*   destruct 1 as (stbl2_rest' & RELOC2' & LINKSTBL1').   *)
+(*   generalize (link_defs_rest_norepet_pres1 _ _ _ _ NORPT1 LINKDEFS1). *)
+(*   intros NORPT1'. *)
+(*   generalize (link_defs1_gen_symbtbl_comm _ _ NORPT1' LINKDEFS2 GSREST2 GSREST1). *)
+(*   destruct 1 as (stbl_linked2 & sr1 & sr2 & LINKSTBL2 & GSLINKED2 & GS3 & GS4). *)
+(*   generalize (reloc_link_symbtable_comm1 _ _ _ RELOC2' LINKSTBL2). *)
+(*   destruct 1 as (stbl2_linked' & RELOC2 & LINKREST2). *)
+
+(*   unfold link_symbtable. *)
+(*   eexists. exists stbl2'. split; auto. *)
+(*   rewrite LINKSTBL1'. *)
+(*   rewrite LINKREST2. split; auto.   *)
+(*   eapply gen_symb_table_reloc_comm; eauto. *)
+(* Qed. *)
+
+
+(** ** Commutativity of linking and section generation *)
+
+Class PERWithFun (A:Type) (aeq:A -> A -> Prop) `{PER A aeq} (f:A -> bool) :=
+{
+  eq_imply_fun_true: forall e1 e2, aeq e1 e2 -> f e1 = true /\ f e2 = true;
+  (** Equality between elements in a restricted domain *)
+  fun_true_imply_eq: forall e, f e = true -> aeq e e;
+}.
+
+Section WithEquivAndFun.
+
+Context `{PERWithFun}.
+
+Inductive list_in_order : list A -> list A -> Prop :=
+| lorder_nil : list_in_order nil nil
+| lorder_left_false : forall e l1 l2, 
+    f e = false -> list_in_order l1 l2 -> list_in_order (e :: l1) l2
+| lorder_right_false : forall e l1 l2,
+    f e = false -> list_in_order l1 l2 -> list_in_order l1 (e :: l2)
+| lorder_true : forall e1 e2 l1 l2,
+    aeq e1 e2 -> list_in_order l1 l2 -> list_in_order (e1::l1) (e2::l2).
+
+Lemma list_in_order_false_inv : forall (l1' l1 l2: list A) e,
+    f e = false -> l1' = (e :: l1) -> list_in_order l1' l2 -> list_in_order l1 l2.
+Proof.
+  induction 3. 
+  - inv H2.
+  - inv H2. auto.
+  - apply lorder_right_false; auto.
+  - subst. inv H2. apply eq_imply_fun_true in H3. destruct H3.
+    congruence.
+Qed.
+
+Lemma list_in_order_true_inv : forall (l1' l1 l2: list A)  e1,
+    f e1 = true -> l1' = (e1 :: l1) -> list_in_order l1' l2 -> 
+    exists l3 l4 e2, l2 = l3 ++ (e2 :: l4) /\ 
+             aeq e1 e2 /\
+             Forall (fun e' => f e' = false) l3 /\
+             list_in_order l1 l4.
+Proof.
+  induction 3.
+  - inv H2.
+  - inv H2. congruence.
+  - subst. 
+    generalize (IHlist_in_order eq_refl).
+    destruct 1 as (l3 & l4 & e2 & EQ & EEQ & FP & ORDER). subst.
+    exists (e :: l3), l4, e2. split.
+    rewrite <- app_comm_cons. auto. split; auto.
+  - inv H2. exists nil, l2, e2. split. auto.
+    split; auto.
+Qed.
+
+Lemma list_in_order_right_false_list : forall (l2' l1 l2: list A),
+    Forall (fun e : A => f e = false) l2' ->
+    list_in_order l1 l2 -> 
+    list_in_order l1 (l2' ++ l2).
+Proof.
+  induction l2'.
+  - intros l1 l2 FALL ORDER. simpl. auto.
+  - intros l1 l2 FALL ORDER. simpl. 
+    generalize (Forall_inv FALL).
+    intros FLS.
+    apply lorder_right_false; auto.
+    apply IHl2'; auto.
+    rewrite Forall_forall in *.
+    intros. apply FALL. apply in_cons. auto.
+Qed.
+
+
+Lemma list_in_order_trans : forall (l1 l2 l3: list A),
+    list_in_order l1 l2 -> list_in_order l2 l3 -> list_in_order l1 l3.
+Proof.
+  intros l1 l2 l3 ORDER.
+  generalize l3.
+  induction ORDER.
+  - auto.
+  - intros l0 ORDER1. constructor; auto.
+  - intros l0 ORDER1. 
+    generalize (list_in_order_false_inv H1 (eq_refl (e::l2)) ORDER1). auto.
+  - intros l0 ORDER1.
+    generalize (eq_imply_fun_true _ _ H1). destruct 1 as (FEQ1 & FEQ2).
+    generalize (list_in_order_true_inv FEQ2 (eq_refl (e2::l2)) ORDER1).
+    destruct 1 as (l2' & l2'' & e3 & EQ & EEQ & ALL & ORDER2).
+    subst.
+    apply IHORDER in ORDER2.
+    apply list_in_order_right_false_list; auto.
+    apply lorder_true; auto.
+    apply PER_Transitive with e2; auto.
+Qed.    
+
+Lemma list_in_order_cons : forall (l1 l2:list A) e,
+    list_in_order l1 l2 -> list_in_order (e::l1) (e::l2).
+Proof.
+  intros l1 l2 e ORDER.
+  destruct (f e) eqn:EQ.
+  - apply lorder_true; auto.
+    apply fun_true_imply_eq. auto.
+  - apply lorder_left_false; auto.
+    apply lorder_right_false; auto.
+Qed.
+
+Lemma list_in_order_refl: forall (l:list A),
+    list_in_order l l.
+Proof.
+  induction l; intros.
+  - apply lorder_nil.
+  - apply list_in_order_cons. auto.
+Qed.
+
+Lemma partition_pres_list_in_order: forall pf (l l1 l2: list A),
+    partition pf l = (l1, l2) ->
+    Forall (fun e => f e = false) l1 ->
+    list_in_order l l2.
+Proof.
+  induction l.
+  - intros l1 l2 PART ALL. simpl in *. inv PART. constructor.
+  - intros l1 l2 PART ALL. simpl in *.
+    destruct (pf a).
+    + destruct (partition pf l) eqn:PART1. inv PART.
+      apply lorder_left_false. 
+      apply Forall_inv in ALL. auto.
+      apply IHl with l0; auto.
+      rewrite Forall_forall in *. intros. 
+      apply ALL; auto. apply in_cons. auto.
+    + destruct (partition pf l) eqn:PART1. inv PART.
+      apply list_in_order_cons. 
+      apply IHl with l1; auto.
+Qed.
+
+End WithEquivAndFun.
+
+Arguments list_in_order [A] _ _ _ _.
+
+
+Section WithFunVar.
+
+Context {F V:Type}.
+
+(** Equality between internal definitions *)
+Definition def_internal (def: option (AST.globdef (AST.fundef F) V)) :=
+  is_def_internal is_fundef_internal def.
+
+Inductive def_eq : 
+  option (AST.globdef (AST.fundef F) V) -> option (AST.globdef (AST.fundef F) V) -> Prop :=
+| fundef_eq : forall f, is_fundef_internal f = true -> def_eq (Some (Gfun f)) (Some (Gfun f))
+| vardef_eq : forall v1 v2, 
+    is_var_internal v1 = true -> is_var_internal v2 = true ->
+    gvar_init v1 = gvar_init v2 -> def_eq (Some (Gvar v1)) (Some (Gvar v2)).
+  
+Lemma def_eq_symm : forall f1 f2, def_eq f1 f2 -> def_eq f2 f1.
+Proof.
+  intros. inv H.
+  - constructor. auto.
+  - econstructor; eauto.
+Qed.
+
+Lemma def_eq_trans: forall f1 f2 f3, 
+    def_eq f1 f2 -> def_eq f2 f3 -> def_eq f1 f3.
+Proof.
+  intros f1 f2 f3 EQ1 EQ2. inv EQ1. 
+  - inv EQ2. constructor. auto.
+  - inv EQ2. econstructor; eauto.
+    eapply eq_trans; eauto.
+Qed.
+
+Lemma def_eq_imply_internal : forall f1 f2,
+    def_eq f1 f2 -> def_internal f1 = true /\ def_internal f2 = true.
+Proof.
+  intros f1 f2 EQ.
+  inv EQ.
+  - simpl. auto.
+  - simpl in *. auto.
+Qed.
+
+Lemma def_internal_imply_eq : 
+  forall f, def_internal f = true -> def_eq f f.
+Proof.
+  intros f INT.
+  destruct f. destruct g.
+  - constructor; auto.
+  - simpl in *. constructor; auto.
+  - simpl in *. congruence.
+Qed.
+
+Instance PERDefEq : PER def_eq :=
+{
+  PER_Symmetric := def_eq_symm;
+  PER_Transitive := def_eq_trans;
+}.
+
+Instance DefEq : PERWithFun def_internal :=
+{
+  eq_imply_fun_true := def_eq_imply_internal;
+  fun_true_imply_eq := def_internal_imply_eq;
+}.
+
+(** Equality between id and internal definition pairs *)
+Definition id_def_internal (iddef: ident * option (AST.globdef (AST.fundef F) V)) :=
+  let '(id, def) := iddef in
+  def_internal def.
+
+Definition id_def_eq (iddef1 iddef2: ident * option (AST.globdef (AST.fundef F) V)) : Prop :=
+  let '(id1, def1) := iddef1 in
+  let '(id2, def2) := iddef2 in
+  id1 = id2 /\ def_eq def1 def2.
+
+Lemma id_def_eq_symm : forall f1 f2, id_def_eq f1 f2 -> id_def_eq f2 f1.
+Proof.
+  intros. unfold id_def_eq in *.
+  destruct f1, f2. destruct H. split; auto.
+  apply def_eq_symm; auto.
+Qed.
+
+Lemma id_def_eq_trans: forall f1 f2 f3, 
+    id_def_eq f1 f2 -> id_def_eq f2 f3 -> id_def_eq f1 f3.
+Proof.
+  intros f1 f2 f3 EQ1 EQ2. 
+  unfold id_def_eq in *. destruct f1, f2, f3.
+  destruct EQ1, EQ2. split.
+  eapply eq_trans; eauto.
+  eapply def_eq_trans; eauto.
+Qed.
+
+Lemma id_def_eq_imply_internal : forall f1 f2,
+    id_def_eq f1 f2 -> id_def_internal f1 = true /\ id_def_internal f2 = true.
+Proof.
+  intros f1 f2 EQ.
+  unfold id_def_eq in EQ.
+  destruct f1, f2. destruct EQ. subst.
+  simpl. 
+  apply def_eq_imply_internal; eauto.
+Qed.
+
+Lemma id_def_interal_imply_eq : 
+  forall f, id_def_internal f = true -> id_def_eq f f.
+Proof.
+  intros f INT.
+  destruct f. destruct o. destruct g.
+  - simpl. split; auto. constructor; auto.
+  - simpl in *. split; auto. constructor; auto.
+  - simpl in *. split; auto. congruence.
+Qed.
+
+Instance PERIdDefEq : PER id_def_eq :=
+{
+  PER_Symmetric := id_def_eq_symm;
+  PER_Transitive := id_def_eq_trans;
+}.
+
+Instance IdDefEq : PERWithFun id_def_internal :=
+{
+  eq_imply_fun_true := id_def_eq_imply_internal;
+  fun_true_imply_eq := id_def_interal_imply_eq;
+}.
+
+
+Lemma link_external_defs : forall {LV: Linker V} (def1 def2 def: option (globdef (AST.fundef F) V)),
+    def_internal def1 = false ->
+    def_internal def2 = false ->
+    link_option def1 def2 = Some def ->
+    def_internal def = false.
+Proof.
+  intros LV def1 def2 def INT1 INT2 LINK.
+  unfold link_option in LINK.
+  destruct def1, def2.
+  - 
+    destruct (link g g0) eqn:LINKG; try congruence. inv LINK.
+    unfold link in LINKG.
+    Transparent Linker_def.
+    unfold Linker_def in LINKG.
+    unfold link_def in LINKG.
+    destruct g, g0.
+    + destruct (link f f0) eqn:LINKF; try congruence. inv LINKG.
+      unfold link in LINKF.
+      Transparent Linker_fundef.
+      unfold Linker_fundef in LINKF.
+      simpl in *.
+      apply link_external_fundefs with f f0; eauto.
+    + congruence.
+    + congruence.
+    + destruct (link v v0) eqn:LINKV; try congruence. inv LINKG.
+      simpl in *.     
+      apply link_external_vars with _ v v0; eauto.
+  - inv LINK. auto.
+  - inv LINK. auto.
+  - inv LINK. auto.
+Qed.    
+  
+
+Lemma link_internal_external_defs : forall {LV: Linker V} (def1 def2 def: option (globdef (AST.fundef F) V)),
+    def_internal def1 = true ->
+    def_internal def2 = false ->
+    link_option def1 def2 = Some def ->
+    def_eq def def1.
+Proof.
+  intros LV def1 def2 def INT1 INT2 LINK.
+  unfold link_option in LINK.
+  destruct def1, def2.
+  - destr_in LINK. inv LINK. simpl in *.
+    destruct g, g0; simpl in *; try congruence.
+    + destr_in Heqo. inv Heqo.
+      generalize (link_extern_fundef_inv _ _ INT2 Heqo0). 
+      intros. subst. constructor. auto.
+    + destr_in Heqo. inv Heqo.
+      generalize (link_internal_external_vars _ _ _ INT1 INT2 Heqo0).
+      destruct 1.
+      constructor; auto.
+  - inv LINK. apply def_internal_imply_eq; auto.
+  - simpl in *. congruence.
+  - simpl in *. congruence.
+Qed.  
+
+
+  
+(* Lemma link_defs1_in_order : forall {LV: Linker V} defs1 defs2 defs1_linked defs1_rest defs2_rest, *)
+(*     list_norepet (map fst defs2) -> *)
+(*     link_defs1 is_fundef_internal defs1 defs2 = Some (defs1_linked, defs1_rest, defs2_rest) -> *)
+(*     list_in_order id_def_eq id_def_internal defs1 defs1_linked /\ *)
+(*     list_in_order id_def_eq id_def_internal defs2 defs2_rest. *)
+(* Proof. *)
+(*   induction defs1 as [|def1 defs1']. *)
+(*   - intros defs2 defs1_linked defs1_rest defs2_rest NORPT LINK. *)
+(*     simpl in *. inv LINK. split. *)
+(*     constructor. *)
+(*     apply list_in_order_refl. *)
+
+(*   - intros defs2 defs1_linked defs1_rest defs2_rest NORPT LINK. *)
+(*     simpl in LINK. destruct def1 as (id1, def1). *)
+(*     destruct (link_defs1 is_fundef_internal defs1' defs2) eqn:LINK1; try congruence. *)
+(*     destruct p as (p, defs2_rest'). *)
+(*     destruct p as (defs1_linked', defs1_rest'). *)
+(*     destruct (partition (fun '(id', _) => ident_eq id' id1) defs2_rest') as (defs2' & defs2_rest'') eqn:PART. *)
+(*     destruct defs2' as [| iddef2 defs2'']. *)
+(*     + (** No definition with the same id found in defs2 *) *)
+(*       inv LINK. *)
+(*       generalize (IHdefs1' _ _ _ _ NORPT LINK1). *)
+(*       destruct 1 as (LORDER1 & LORDER2). *)
+(*       split; auto.       *)
+(*       apply list_in_order_cons; eauto. *)
+
+(*     + (** Some definition with the same id found in defs2 *) *)
+(*       destruct iddef2 as (id2 & def2).      *)
+(*       destruct (is_def_internal_dec is_fundef_internal def2) as [DEFINT2 | DEFINT2]; *)
+(*         rewrite DEFINT2 in LINK. *)
+(*       destruct (is_def_internal_dec is_fundef_internal def1) as [DEFINT1 | DEFINT1]; *)
+(*         rewrite DEFINT1 in LINK. *)
+(*       congruence. *)
+(*       inv LINK. *)
+(*       * (** The left definition is external and the right definition is internal. *)
+(*             The linking is delayed *) *)
+(*         generalize (IHdefs1' _ _ _ _ NORPT LINK1). *)
+(*         destruct 1 as (LORDER1 & LORDER2). split; auto. *)
+(*         apply lorder_left_false; auto. *)
+
+(*       * destruct (link_option def1 def2) as [def|] eqn:LINK_SYMB; inv LINK. *)
+(*         (** The right definition is external. *)
+(*             The linking proceeds normally *) *)
+(*         generalize (IHdefs1' _ _ _ _ NORPT LINK1). *)
+(*         destruct 1 as (LORDER1 & LORDER2). *)
+(*         generalize (link_defs_rest_norepet_pres2 _ is_fundef_internal _ _ NORPT LINK1). *)
+(*         intros NORPT1. *)
+(*         generalize (lst_norepet_partition_inv _ _ NORPT1 PART). *)
+(*         destruct 1. congruence. destruct H. inv H. *)
+(*         subst. split. *)
+(*         ** destruct (def_internal def1) eqn:DEFINT1. *)
+(*            *** generalize (link_internal_external_defs _ def2 DEFINT1 DEFINT2 LINK_SYMB). *)
+(*                intros DEQ.  *)
+(*                apply lorder_true. simpl. split; auto. *)
+(*                apply PER_Symmetric; auto. *)
+(*                auto. *)
+(*            *** simpl in LINK_SYMB. inv LINK_SYMB. *)
+(*                apply lorder_left_false; auto. *)
+(*                apply lorder_right_false; auto. *)
+(*                simpl.  *)
+(*                apply link_external_defs with def1 def2; eauto. *)
+(*         ** generalize (partition_pres_list_in_order _ _ PART). *)
+(*            intros LORDER3. *)
+(*            apply list_in_order_trans with defs2_rest'; auto. *)
+(* Qed. *)
+
+End WithFunVar.
+(** *)
+
+Axiom defs_size_inbound: forall defs, sections_size (create_sec_table defs) <= Ptrofs.max_unsigned.
+
+(** Data section generation and linking *)
+
+Lemma extern_var_init_data_nil : forall v,
+    is_var_internal v = false ->
+    get_def_init_data (Some (Gvar v)) = [].
+Proof.
+  intros v H. simpl in *.
+  unfold is_var_internal in H.
+  destruct (gvar_init v); try congruence.
+  destruct i; simpl in *; try congruence.
+  destruct l; simpl in *; try congruence.
+Qed.
+
+Lemma extern_init_data_nil : forall def,
+    def_internal def = false -> get_def_init_data def = nil.
+Proof.
+  intros def H.
+  destruct def. destruct g. 
+  - simpl in *. auto.
+  - simpl in H. apply extern_var_init_data_nil. auto.
+  - simpl in *. auto.
+Qed.
+
+
+Lemma acc_init_data_app : forall def l1 l2,
+    (acc_init_data def l1) ++ l2 = acc_init_data def (l1 ++ l2).
+Proof.
+  intros def l1 l2. destruct def as (id & def').
+  simpl. rewrite app_assoc. auto.
+Qed.
+
+Lemma fold_right_acc_init_data_app : forall defs l,
+    fold_right acc_init_data [] defs ++ l = fold_right acc_init_data l defs.
+Proof.
+  induction defs. 
+  - intros l. simpl. auto.
+  - intros l. simpl. 
+    rewrite acc_init_data_app. rewrite IHdefs. auto.
+Qed.
+
+Lemma get_def_init_data_eq : forall d1 d2,
+      def_eq d1 d2 -> get_def_init_data d1 = get_def_init_data d2.
+Proof.
+  intros d1 d2 EQ. inv EQ.
+  - simpl. auto.
+  - simpl in *. rewrite H1. auto.
+Qed.
+
+Lemma acc_init_data_eq: forall d1 d2 l,
+    id_def_eq d1 d2 -> acc_init_data d1 l = acc_init_data d2 l.
+Proof.
+  intros d1 d2 l EQ.
+  destruct d1, d2. simpl in *. destruct EQ. subst.
+  f_equal. apply get_def_init_data_eq. auto.
+Qed.
+
+Lemma acc_init_data_in_order_eq : forall defs1 defs2,
+    list_in_order id_def_eq id_def_internal defs1 defs2 ->
+    fold_right acc_init_data [] defs1 = fold_right acc_init_data [] defs2.
+Proof.
+  induction 1.
+  - simpl. auto.
+  - destruct e as (id, def). simpl.     
+    erewrite extern_init_data_nil; eauto.
+  - destruct e as (id, def). simpl.
+    erewrite extern_init_data_nil; eauto.
+  - simpl.
+    rewrite IHlist_in_order. auto.
+    apply acc_init_data_eq; auto.
+Qed.          
+
+(** Hint for Asm definitions *)                
+Definition PERIdAsmDefEq := (@PERIdDefEq Asm.function unit).
+Existing Instance PERIdAsmDefEq.
+Definition IdAsmDefEq := (@IdDefEq Asm.function unit).
+Existing Instance IdAsmDefEq.
+
+(* Lemma link_acc_init_data_comm : forall defs1 defs2 defs, *)
+(*     list_norepet (map fst defs1) -> *)
+(*     list_norepet (map fst defs2) -> *)
+(*     link_defs is_fundef_internal defs1 defs2 = Some defs -> *)
+(*     fold_right acc_init_data [] defs =  *)
+(*     fold_right acc_init_data [] defs1 ++ fold_right acc_init_data [] defs2. *)
+(* Proof. *)
+(*   intros defs1 defs2 defs NORPT1 NORPT2 LINK. *)
+(*   unfold link_defs in LINK. *)
+(*   destruct (link_defs1 is_fundef_internal defs1 defs2) eqn:LINK1; try inv LINK. *)
+(*   destruct p as (r & defs2_rest). destruct r as (defs1_linked & defs1_rest). *)
+(*   destruct (link_defs1 is_fundef_internal defs2_rest defs1_rest) eqn:LINK2; try inv H0. *)
+(*   destruct p. destruct p as (defs2_linked & p). inv H1. *)
+(*   rewrite fold_right_app. rewrite <- fold_right_acc_init_data_app. *)
+(*   generalize (link_defs_rest_norepet_pres1 _ is_fundef_internal defs1 defs2 NORPT1 LINK1). *)
+(*   intros NORPT3. *)
+(*   apply link_defs1_in_order in LINK1; auto. destruct LINK1 as (ORDER1 & ORDER2). *)
+(*   apply link_defs1_in_order in LINK2; auto. destruct LINK2 as (ORDER3 & ORDER4). *)
+(*   generalize (list_in_order_trans ORDER2 ORDER3). *)
+(*   intros ORDER5. *)
+(*   rewrite (acc_init_data_in_order_eq ORDER1). *)
+(*   rewrite (acc_init_data_in_order_eq ORDER5). auto.   *)
+(* Qed. *)
+
+
+(** Code section generation and linking *)
+Lemma extern_fun_nil : forall def,
+    def_internal def = false -> get_def_instrs def = nil.
+Proof.
+  intros def H.
+  destruct def. destruct g; simpl in *.
+  - unfold is_fundef_internal in H.
+    destruct f; try congruence.
+  - auto.
+  - simpl in *. auto.
+Qed.
+
+Lemma acc_instrs_app : forall def l1 l2,
+    (acc_instrs def l1) ++ l2 = acc_instrs def (l1 ++ l2).
+Proof.
+  intros def l1 l2. destruct def as (id & def').
+  simpl. rewrite app_assoc. auto.
+Qed.
+
+Lemma fold_right_acc_instrs_app : forall defs l,
+    fold_right acc_instrs [] defs ++ l = fold_right acc_instrs l defs.
+Proof.
+  induction defs. 
+  - intros l. simpl. auto.
+  - intros l. simpl. 
+    rewrite acc_instrs_app. rewrite IHdefs. auto.
+Qed.
+
+Lemma get_def_instrs_eq : forall d1 d2,
+      def_eq d1 d2 -> get_def_instrs d1 = get_def_instrs d2.
+Proof.
+  intros d1 d2 EQ. inv EQ.
+  - auto.
+  - simpl in *. auto.
+Qed.
+
+Lemma acc_instrs_eq: forall d1 d2 l,
+    id_def_eq d1 d2 -> acc_instrs d1 l = acc_instrs d2 l.
+Proof.
+  intros d1 d2 l EQ.
+  destruct d1, d2. simpl in *. destruct EQ. subst.
+  f_equal. apply get_def_instrs_eq. auto.
+Qed.
+
+Lemma acc_instrs_in_order_eq : forall defs1 defs2,
+    list_in_order id_def_eq id_def_internal defs1 defs2 ->
+    fold_right acc_instrs [] defs1 = fold_right acc_instrs [] defs2.
+Proof.
+  induction 1.
+  - simpl. auto.
+  - destruct e as (id, def). simpl.     
+    erewrite extern_fun_nil; eauto.
+  - destruct e as (id, def). simpl.
+    erewrite extern_fun_nil; eauto.
+  - simpl.
+    rewrite IHlist_in_order.
+    apply acc_instrs_eq; auto.
+Qed.
+
+
+(* Lemma link_acc_instrs_comm : forall defs1 defs2 defs, *)
+(*     list_norepet (map fst defs1) -> *)
+(*     list_norepet (map fst defs2) -> *)
+(*     link_defs is_fundef_internal defs1 defs2 = Some defs -> *)
+(*     fold_right acc_instrs [] defs =  *)
+(*     (fold_right acc_instrs [] defs1) ++ (fold_right acc_instrs [] defs2). *)
+(* Proof. *)
+(*   intros defs1 defs2 defs NORPT1 NORPT2 LINK. *)
+(*   unfold link_defs in LINK. *)
+(*   destruct (link_defs1 is_fundef_internal defs1 defs2) eqn:LINK1; try inv LINK. *)
+(*   destruct p as (r & defs2_rest). destruct r as (defs1_linked & defs1_rest). *)
+(*   destruct (link_defs1 is_fundef_internal defs2_rest defs1_rest) eqn:LINK2; try inv H0. *)
+(*   destruct p. destruct p as (defs2_linked & p). inv H1. *)
+(*   rewrite fold_right_app. rewrite <- fold_right_acc_instrs_app. *)
+(*   generalize (link_defs_rest_norepet_pres1 _ is_fundef_internal defs1 defs2 NORPT1 LINK1). *)
+(*   intros NORPT3. *)
+(*   apply link_defs1_in_order in LINK1; auto. destruct LINK1 as (ORDER1 & ORDER2). *)
+(*   apply link_defs1_in_order in LINK2; auto. destruct LINK2 as (ORDER3 & ORDER4). *)
+(*   generalize (list_in_order_trans ORDER2 ORDER3). *)
+(*   intros ORDER5. *)
+(*   rewrite (acc_instrs_in_order_eq ORDER1). *)
+(*   rewrite (acc_instrs_in_order_eq ORDER5). auto.   *)
+(* Qed. *)
+
+(** Symbol table size *)
+Lemma init_data_list_size_app : forall l1 l2,
+    init_data_list_size (l1 ++ l2) = (init_data_list_size l1) + (init_data_list_size l2).
+Proof.
+  induction l1 as [| e l2'].
+  - intros l2. simpl. auto.
+  - intros l2. simpl in *.
+    rewrite IHl2'; omega.
+Qed.
+
+Lemma code_size_app: forall l1 l2,
+    code_size (l1 ++ l2) = code_size l1 + code_size l2.
+Proof.
+  induction l1 as [| e l2'].
+  - intros l2. simpl. auto.
+  - intros l2. simpl in *.
+    rewrite IHl2'; omega.
+Qed.
+
+Lemma update_code_data_size_inv : forall def dsz csz dincr cincr,
+    dincr = init_data_list_size (get_def_init_data def) ->
+    cincr = code_size (get_def_instrs def) ->
+    update_code_data_size dsz csz def = (dincr + dsz, cincr + csz).
+Proof.
+  intros def dsz csz dincr cincr DINCR CINCR.
+  unfold update_code_data_size. destruct def. destruct g. destruct f.
+  - simpl in *. subst. f_equal; omega.
+  - simpl in *. subst. f_equal; omega.
+  - simpl in DINCR, CINCR. subst.
+    destruct (gvar_init v).
+    + simpl. auto.
+    + destruct i; try (f_equal; omega).
+      destruct l; f_equal; omega.
+  - simpl in *. subst. f_equal; omega.
+Qed.
+
+Lemma acc_symb_size: forall d_id c_id defs s1 s2 dsz1 csz1 dsz2 csz2 data code,
+    fold_left (acc_symb d_id c_id) defs (s1, dsz1, csz1) = (s2, dsz2, csz2) ->
+    init_data_list_size data = dsz1 ->
+    code_size code = csz1 ->
+    init_data_list_size (fold_right acc_init_data data defs) = dsz2 /\ 
+    code_size (fold_right acc_instrs code defs) = csz2.
+Proof.
+  induction defs as [| def defs].
+  - intros s1 s2 dsz1 csz1 dsz2 csz2 data code SYMB INIT CODE.
+    simpl in *. inv SYMB. auto.
+  - intros s1 s2 dsz1 csz1 dsz2 csz2 data code SYMB INIT CODE.
+    destruct def as (id, def).
+    simpl in *. destr_in SYMB.
+    rewrite init_data_list_size_app.
+    rewrite code_size_app.
+    erewrite update_code_data_size_inv in Heqp; eauto.
+    inv Heqp.
+    rewrite <- init_data_list_size_app in SYMB.
+    rewrite <- code_size_app in SYMB.
+    generalize (IHdefs _ _ _ _ _ _ _ _ SYMB 
+                       (@eq_refl _ (init_data_list_size (get_def_init_data def ++ data)))
+                       (@eq_refl _ (code_size (get_def_instrs def ++ code)))).
+    destruct 1. subst. split.
+    + rewrite <- (fold_right_acc_init_data_app defs data).
+      rewrite <- (fold_right_acc_init_data_app defs (get_def_init_data def ++ data)).
+      repeat rewrite init_data_list_size_app.
+      omega.
+    + rewrite <- (fold_right_acc_instrs_app defs code).
+      rewrite <- (fold_right_acc_instrs_app defs (get_def_instrs def ++ code)).
+      repeat rewrite code_size_app.
+      omega.
+Qed.
+
+
+Lemma gen_symb_table_size: forall defs d_id c_id stbl dsz csz,
+    gen_symb_table d_id c_id defs = (stbl, dsz, csz) ->
+    sec_size (create_data_section defs) = dsz /\
+    sec_size (create_code_section defs) = csz.
+Proof.
+  intros defs d_id c_id stbl dsz csz SGEN.
+  simpl. unfold gen_symb_table in SGEN.
+  destr_in SGEN. destruct p. inv SGEN. 
+  eapply acc_symb_size; eauto.
+Qed.
+
+
+(** ** Main linking theorem *)
+(* Lemma link_transf_symbtablegen : forall (p1 p2 : Asm.program) (tp1 tp2 : program) (p : Asm.program), *)
+(*     link p1 p2 = Some p -> match_prog p1 tp1 -> match_prog p2 tp2 ->  *)
+(*     exists tp : program, link tp1 tp2 = Some tp /\ match_prog p tp. *)
+(* Proof. *)
+(*   intros p1 p2 tp1 tp2 p LINK MATCH1 MATCH2. *)
+(*   unfold link. unfold Linker_reloc_prog. unfold link_reloc_prog. *)
+(*   rewrite <- (match_prog_pres_prog_defs MATCH1). *)
+(*   rewrite <- (match_prog_pres_prog_defs MATCH2). *)
+(*   rewrite <- (match_prog_pres_prog_main MATCH1). *)
+(*   rewrite <- (match_prog_pres_prog_main MATCH2). *)
+(*   rewrite <- (match_prog_pres_prog_public MATCH1). *)
+(*   rewrite <- (match_prog_pres_prog_public MATCH2). *)
+(*   setoid_rewrite LINK. *)
+(*   apply link_prog_inv in LINK. *)
+(*   destruct LINK as (MAINEQ & NRPT1 & NRPT2 & defs & PEQ & LINKDEFS). subst. simpl. *)
+(*   unfold match_prog in *. *)
+
+(*   unfold transf_program in MATCH1. *)
+(*   destruct check_wellformedness; try monadInv MATCH1. *)
+(*   destruct (gen_symb_table sec_data_id sec_code_id (AST.prog_defs p1)) as (p & csz1) eqn:GSEQ1 . *)
+(*   destruct p as (stbl1 & dsz1). *)
+(*   destruct zle; try monadInv MATCH1; simpl. *)
+  
+(*   unfold transf_program in MATCH2. *)
+(*   destruct check_wellformedness; try monadInv MATCH2. *)
+(*   destruct (gen_symb_table sec_data_id sec_code_id (AST.prog_defs p2)) as (p & csz2) eqn:GSEQ2 . *)
+(*   destruct p as (stbl2 & dsz2). *)
+(*   destruct zle; try monadInv MATCH2; simpl. *)
+  
+(*   generalize (link_gen_symb_comm _ _ NRPT1 NRPT2 LINKDEFS GSEQ1 GSEQ2  *)
+(*                                  (@eq_refl _ (reloc_offset_fun dsz1 csz1))); eauto. *)
+(*   destruct 1 as (stbl & stbl2' & RELOC & LINKS & GENS). *)
+(*   generalize (gen_symb_table_size _ _ _ GSEQ1). *)
+(*   destruct 1 as (DSZ & CSZ). *)
+(*   setoid_rewrite DSZ. *)
+(*   setoid_rewrite CSZ. *)
+(*   rewrite RELOC. *)
+(*   unfold reloc_iter. cbn. *)
+(*   rewrite LINKS. *)
+
+(*   eexists. split. reflexivity. *)
+(*   unfold transf_program. *)
+
+(*   exploit link_pres_wf_prog; eauto. *)
+(*   intros WF. *)
+(*   destruct check_wellformedness; try congruence. *)
+(*   simpl. rewrite GENS. *)
+  
+(*   destruct zle. *)
+(*   repeat f_equal. *)
+(*   unfold create_sec_table. repeat f_equal. *)
+(*   unfold create_data_section. f_equal. *)
+(*   apply link_acc_init_data_comm; auto. *)
+(*   unfold create_code_section. f_equal. *)
+(*   apply link_acc_instrs_comm; auto. *)
+(*   generalize (defs_size_inbound defs). *)
+(*   intros; omega. *)
+(* Qed. *)
+
+Existing Instance Linker_prog_ordered.
+
+Lemma link_transf_symbtablegen : forall (p1 p2 : Asm.program) (tp1 tp2 : program) (p : Asm.program),
+    link p1 p2 = Some p -> match_prog p1 tp1 -> match_prog p2 tp2 ->
+    exists tp : program, link tp1 tp2 = Some tp /\ match_prog p tp.
+Proof.
+  cbn in *.
+  Admitted.
+
+Instance TransfLinkSymbtablegen : TransfLink match_prog :=
+  link_transf_symbtablegen.
